work on correctness

NLustreToSyBloc/Correctness.v
@@ -38,7 +38,7 @@ Module Type CORRECTNESS
        (Import Clks    : CLOCKS          Ids)
        (Import ExprSyn : NLEXPRSYNTAX        Op)
        (Import SynNL   : NLSYNTAX        Ids Op       Clks ExprSyn)
-       (SynSB          : SBSYNTAX        Ids Op       Clks ExprSyn)
+       (Import SynSB          : SBSYNTAX        Ids Op       Clks ExprSyn)
        (Import Str     : STREAM              Op OpAux)
        (Import Ord     : ORDERED         Ids Op       Clks ExprSyn SynNL)
        (Import ExprSem : NLEXPRSEMANTICS Ids Op OpAux Clks ExprSyn             Str)
@@ -66,10 +66,10 @@ Module Type CORRECTNESS
   (* Definition inst_in_eqs (x: ident) (eqs: list SynSB.equation) : Prop := *)
   (*   List.Exists (inst_in_eq x) eqs. *)
 
-  Inductive well_formed_app_eq: equation -> Prop :=
+  Inductive well_formed_app_eq: SynNL.equation -> Prop :=
   | wfa_EqDef:
       forall x ck e,
-        well_formed_app_eq (EqDef x ck e)
+        well_formed_app_eq (SynNL.EqDef x ck e)
   | wfa_EqFby:
       forall x ck v0 e,
         well_formed_app_eq (EqFby x ck v0 e)
@@ -369,10 +369,201 @@ Module Type CORRECTNESS
   (*   - unfold SemSB.restr_hist, PM.map; simpl; rewrite PM.gmapi, Find'; auto. *)
   (* Qed. *)
 
+  Lemma In_fst_fold_left_gather_eq:
+    forall eqs xc mems insts,
+      In xc (fst (fold_left gather_eq eqs (mems, insts))) <->
+      In xc mems \/ In xc (fst (fold_left gather_eq eqs ([], insts))).
+  Proof.
+    induction eqs as [|[]]; simpl; intros; auto.
+    - split; auto; intros [|]; auto; contradiction.
+    - destruct i; simpl in *; auto.
+    - rewrite IHeqs; symmetry; rewrite IHeqs.
+      split; intros [Hin|Hin']; auto.
+      + now left; right.
+      + destruct Hin' as [[|]|]; auto; try contradiction.
+        now left; left.
+      + destruct Hin; auto.
+        now right; left; left.
+  Qed.
+
+  Lemma In_snd_fold_left_gather_eq:
+    forall eqs xf mems insts,
+      In xf (snd (fold_left gather_eq eqs (mems, insts))) <->
+      In xf insts \/ In xf (snd (fold_left gather_eq eqs (mems, []))).
+  Proof.
+    induction eqs as [|[]]; simpl; intros; auto.
+    - split; auto; intros [|]; auto; contradiction.
+    - destruct i; simpl in *; auto.
+      rewrite IHeqs; symmetry; rewrite IHeqs.
+      split; intros [Hin|Hin']; auto.
+      + now left; right.
+      + destruct Hin' as [[|]|]; auto; try contradiction.
+        now left; left.
+      + destruct Hin; auto.
+        now right; left; left.
+  Qed.
+
+  Lemma In_snd_gather_eqs_Is_node_in:
+    forall eqs i f,
+      In (i, f) (snd (gather_eqs eqs)) ->
+      Is_node_in f eqs.
+  Proof.
+    unfold gather_eqs.
+    intro.
+    generalize (@nil (ident * const)).
+    induction eqs as [|[]]; simpl; try contradiction; intros ** Hin; auto.
+    - right; eapply IHeqs; eauto.
+    - destruct i.
+      + right; eapply IHeqs; eauto.
+      + apply In_snd_fold_left_gather_eq in Hin as [Hin|Hin].
+        * destruct Hin as [E|]; try contradiction; inv E.
+          left; constructor.
+        * right; eapply IHeqs; eauto.
+    - right; eapply IHeqs; eauto.
+  Qed.
+
+  Lemma Ordered_nodes_blocks:
+    forall G,
+      Ordered_nodes G ->
+      Ordered_blocks (translate G).
+  Proof.
+    induction 1 as [|??? IH NodeIn Nodup]; simpl; constructor; auto.
+    - destruct nd; simpl in *; clear - NodeIn.
+      apply Forall_forall; intros ** Hin.
+      destruct x; apply In_snd_gather_eqs_Is_node_in in Hin.
+      apply NodeIn in Hin as [? E]; split; auto.
+      clear NodeIn.
+      induction nds as [|n].
+      + inv E.
+      + simpl; destruct (ident_eqb (n_name n) i0) eqn: Eq.
+        * inv E; eauto.
+        * inv E; eauto.
+          rewrite ident_eqb_refl in Eq; discriminate.
+    - clear - Nodup.
+      induction Nodup; simpl; auto.
+  Qed.
+
+  Lemma msem_eqs_reset_lasts:
+    forall G bk H M M' n,
+      memory_closed_n M (n_eqs n) ->
+      Forall (msem_equation G bk H M M') (n_eqs n) ->
+      reset_lasts (translate_node n) (M 0).
+  Proof.
+    intros ** Closed Heqs.
+    split.
+    - intros ** Hin.
+      destruct n; simpl in *.
+      unfold gather_eqs in *.
+      clear - Heqs Hin.
+      revert Hin; generalize (@nil (ident * ident)).
+      induction n_eqs0 as [|[] ? IH]; simpl in *; intros; try contradiction;
+        inversion_clear Heqs as [|?? Heq]; inv Heq; eauto.
+      + destruct i; try discriminate; eauto.
+      + destruct i; try discriminate; eauto.
+      + apply In_fst_fold_left_gather_eq in Hin as [Hin|]; eauto.
+        destruct Hin as [E|]; try contradiction; inv E.
+        match goal with H: mfby _ _ _ _ _ _ |- _ => destruct H as (?&?) end; auto.
+    - specialize (Closed 0); destruct Closed as [? Vals].
+      intros ** Find.
+      assert (In x (SynNL.gather_mem (n_eqs n))) as Hin
+          by (apply Vals, not_None_is_Some; eauto).
+      destruct n; simpl in *.
+      unfold gather_eqs in *.
+      clear - Hin Find Heqs.
+      revert Hin; generalize (@nil (ident * ident)).
+      induction n_eqs0 as [|[] ? IH]; simpl in *; intros; try contradiction;
+        inversion_clear Heqs as [|?? Heq]; inv Heq; eauto.
+      + destruct i; try discriminate; eauto.
+      + destruct i; try discriminate; eauto.
+      + destruct Hin.
+        * subst.
+          match goal with H: mfby _ _ _ _ _ _ |- _ => destruct H as (Find'&?) end.
+          rewrite Find in Find'; inv Find'.
+          exists c0; split; auto.
+          apply In_fst_fold_left_gather_eq; left; left; auto.
+        * edestruct IH as (c1 &?& Hin); eauto.
+          exists c1; split; auto.
+          apply In_fst_fold_left_gather_eq; right; eauto.
+  Qed.
+
+  Lemma msem_eqs_In_snd_gather_eqs_spec:
+    forall eqs G bk H M M' x f,
+      Forall (msem_equation G bk H M M') eqs ->
+      In (x, f) (snd (gather_eqs eqs)) ->
+      exists xss Mx Mx' yss,
+        (msem_node G f xss Mx Mx' yss
+         \/ exists r, msem_reset G f r xss Mx Mx' yss)
+        /\ sub_inst_n x M Mx.
+  Proof.
+    unfold gather_eqs.
+    intro; generalize (@nil (ident * const)).
+    induction eqs as [|[]]; simpl; intros ** Heqs Hin;
+      inversion_clear Heqs as [|?? Heq];
+      try inversion_clear Heq as [|????????????? Hd|????????????????? Hd|];
+        try contradiction; eauto.
+    - destruct i; try discriminate.
+      apply In_snd_fold_left_gather_eq in Hin as [Hin|]; eauto.
+      destruct Hin as [E|]; try contradiction; inv E; inv Hd.
+      do 4 eexists; split; eauto.
+    - destruct i; try discriminate.
+      apply In_snd_fold_left_gather_eq in Hin as [Hin|]; eauto.
+      destruct Hin as [E|]; try contradiction; inv E; inv Hd.
+      do 4 eexists; split; eauto.
+  Qed.
+
+  Lemma msem_node_initial_state:
+    forall G f xss M M' yss,
+      Ordered_nodes G ->
+      msem_node G f xss M M' yss ->
+      initial_state (translate G) f (M 0).
+  Proof.
+    induction G as [|node ? IH].
+    inversion 2;
+      match goal with Hf: find_node _ [] = _ |- _ => inversion Hf end.
+    intros ** Hord Hsem.
+    assert (Hsem' := Hsem).
+    inversion_clear Hsem' as [???????? Clock Hfind Ins ???? Heqs].
+    pose proof (find_node_not_Is_node_in _ _ _ Hord Hfind) as Hnini.
+    pose proof Hord; inversion_clear Hord as [|??? NodeIn].
+    pose proof Hfind as Hfind'.
+    simpl in Hfind.
+    assert (Ordered_blocks (translate_node node :: translate G))
+           by (change (translate_node node :: translate G) with (translate (node :: G));
+               apply Ordered_nodes_blocks; auto).
+    destruct (ident_eqb node.(n_name) f) eqn:Hnf.
+    - inversion Hfind; subst n.
+      apply find_node_translate in Hfind' as (?&?&?&?); subst.
+      eapply Forall_msem_equation_global_tl in Heqs; eauto.
+      econstructor; eauto.
+      + eapply msem_eqs_reset_lasts; eauto.
+      + intros ** Hin.
+        assert (b' <> n_name node).
+        { destruct node; simpl in *.
+          apply In_snd_gather_eqs_Is_node_in in Hin.
+          apply NodeIn; auto.
+        }
+        destruct node; simpl in *.
+        edestruct msem_eqs_In_snd_gather_eqs_spec
+          as (?& Mx &?&?& [Node|(rs & Reset)] & Sub); eauto.
+        * apply IH in Node; auto.
+          eexists; split; eauto.
+          apply initial_state_tail; simpl; auto.
+        * inversion_clear Reset as [?????? Nodes].
+          destruct (Nodes (count rs 0)) as (M0 &?& Node & Mmask &?).
+          apply IH in Node; auto.
+          specialize (Mmask 0); specialize (Sub 0).
+          rewrite <-Mmask in Sub; auto.
+          eexists; split; eauto.
+          apply initial_state_tail; simpl; auto.
+    - assert (n_name node <> f) by now apply ident_eqb_neq.
+      eapply msem_node_cons in Hsem; eauto.
+      simpl; rewrite <-initial_state_tail; eauto.
+  Qed.
+
   Section Global.
 
-    Variable G: SynNL.global.
-    Let P := translate G.
+    (* Variable G: global. *)
+    (* Let P := translate G. *)
 
     (*   Inductive lasts_eq_spec (lasts: Env.t const) : equation -> Prop := *)
     (* | LSdef: *)
@@ -390,44 +581,21 @@ Module Type CORRECTNESS
 
 
     Definition sem_equations_n
-               (P: SynSB.program) (bk: stream bool) (H: history)
-               (E: stream SemSB.state) (T: stream SemSB.transient_states) (E': stream SemSB.state)
-               (eqs: list SynSB.equation) :=
-      forall n, Forall (SemSB.sem_equation P (bk n) (restr_hist H n) (E n) (T n) (E' n)) eqs.
+               (P: program) (bk: stream bool) (H: history)
+               (E: stream state) (T: stream transient_states) (E': stream state)
+               (eqs: list equation) :=
+      forall n, Forall (sem_equation P (bk n) (restr_hist H n) (E n) (T n) (E' n)) eqs.
 
     Definition sem_block_n
-               (P: SynSB.program) (f: ident)
-               (E: stream SemSB.state) (xss yss: stream (list value)) (E': stream SemSB.state) :=
-      forall n, SemSB.sem_block P f (E n) (xss n) (yss n) (E' n).
+               (P: program) (f: ident)
+               (E: stream state) (xss yss: stream (list value)) (E': stream state) :=
+      forall n, sem_block P f (E n) (xss n) (yss n) (E' n).
 
-    (* Definition sem_reset_n *)
-    (*            (P: SynSB.program) (f: ident) (r: stream bool) (E E0: stream SemSB.state) := *)
-    (*   forall n, SemSB.sem_reset P f (r n) (E n) (E0 n). *)
-
-    (* Definition entry_states (M M': memories) : stream SemSB.state := *)
-    (*   fun n => match n with *)
-    (*         | 0 => M 0 *)
-    (*         | S n => M' n *)
-    (*         end. *)
-
-    (* Definition instances_n (M: memories) : stream SemSB.transient_states := *)
-    (*   fun n => instances (M n). *)
-
-    (* Lemma entry_states_sub_inst_n: *)
-    (*   forall M M' x Mx Mx', *)
-    (*     sub_inst_n x M Mx -> *)
-    (*     sub_inst_n x M' Mx' -> *)
-    (*     sub_inst_n x (entry_states M M') (entry_states Mx Mx'). *)
-    (* Proof. *)
-    (*   intros ** S S' n. *)
-    (*   destruct n; simpl; auto. *)
-    (* Qed. *)
-
-    Definition add_n (x: ident) (Mx: stream SemSB.state) (I: stream SemSB.transient_states) :=
+    Definition add_n (x: ident) (Mx: stream state) (I: stream transient_states) :=
       fun n => Env.add x (Mx n) (I n).
 
     Lemma sem_equations_n_add_n:
-      forall eqs bk H S S' Is x Sx,
+      forall P eqs bk H S S' Is x Sx,
         sem_equations_n P bk H S Is S' eqs ->
         sem_equations_n P bk H S (add_n x Sx Is) S' eqs.
     Proof.
@@ -445,14 +613,14 @@ Module Type CORRECTNESS
     Qed.
 
     Lemma equation_correctness:
-      forall eq eqs bk H M M' Is,
+      forall G eq eqs bk H M M' Is,
         (forall f xss M M' yss,
             msem_node G f xss M M' yss ->
-            sem_block_n P f M xss yss M') ->
+            sem_block_n (translate G) f M xss yss M') ->
         Ordered_nodes G ->
         msem_equation G bk H M M' eq ->
-        sem_equations_n P bk H M Is M' eqs ->
-        exists Is', sem_equations_n P bk H M Is' M' (translate_eqn eq ++ eqs).
+        sem_equations_n (translate G) bk H M Is M' eqs ->
+        exists Is', sem_equations_n (translate G) bk H M Is' M' (translate_eqn eq ++ eqs).
     Proof.
       intros ** IHnode Hord Heq Heqs.
       destruct Heq as [| |?????????????????????? Var Hr Reset|?????????? Arg Var Mfby];
@@ -473,21 +641,13 @@ Module Type CORRECTNESS
         exists (fun n => Env.add x (if rs n then Mx 0 else Mx n) (Is n)); intro.
         pose proof (msem_reset_spec Hord Reset) as Spec.
         inversion_clear Reset as [?????? Nodes].
-        assert (forall k, exists Mk Mk',
-                     sem_block_n P f Mk
-                                 (mask (all_absent (ls 0)) k rs ls)
-                                 (mask (all_absent (xss 0)) k rs xss)
-                                 Mk'
-                     /\ memory_masked k rs Mx Mk
-                     /\ memory_masked k rs Mx' Mk') as Blocks
-            by (intro; destruct (Nodes k) as (?&?&?&?&?);
-                do 2 eexists; intuition; eauto); clear Nodes.
-        specialize (Blocks (count rs n)).
-        destruct Blocks as (Mk & Mk' & Blocks & Mmask & Mmask').
-        specialize (Blocks n); specialize (Mmask n); specialize (Mmask' n).
-        rewrite 2 mask_transparent, Mmask, Mmask' in Blocks; auto.
+        destruct (Nodes (count rs n)) as (Mn & Mn' & Node_n & Mmask_n & Mmask'_n);
+          destruct (Nodes (count rs 0)) as (M0 & M0' & Node_0 & Mmask_0 & Mmask'_0).
+        apply IHnode in Node_n.
+        specialize (Node_n n); specialize (Mmask_n n); specialize (Mmask'_n n).
+        rewrite 2 mask_transparent, Mmask_n, Mmask'_n in Node_n; auto.
         specialize (Var n); specialize (Hr n).
-        assert (forall Mx, sem_equations_n P bk H M (add_n x Mx Is) M' eqs) as Heqs'
+        assert (forall Mx, sem_equations_n (translate G) bk H M (add_n x Mx Is) M' eqs) as Heqs'
             by now intro; apply sem_equations_n_add_n.
         destruct (rs n) eqn: E.
         + specialize (Heqs' (fun n => Mx 0) n).
@@ -499,7 +659,8 @@ Module Type CORRECTNESS
              - eapply Son; eauto.
                admit.
              - instantiate (1 := empty_memory _); simpl.
-               admit.
+               rewrite <-Mmask_0; auto.
+               eapply msem_node_initial_state; eauto.
            }
           *{ eapply SemSB.SEqCall with (Is := Mx 0); eauto.
              - instantiate (1 := empty_memory _); congruence.
@@ -533,2017 +694,89 @@ Module Type CORRECTNESS
         destruct (ls n); destruct Spec as (?& Hxs); rewrite Hxs in Var; inv Arg'; eauto using sem_equation.
     Qed.
 
-    Theorem correctness:
-      forall f xss M yss,
-        msem_node G f xss M yss ->
-        exists E E',
-        forall n, SemSB.sem_block P f (E n) (xss n) (yss n) (E' n).
-    Proof.
-      intros.
-
-
-    Section Sem.
-
-      Variable bk: stream bool.
-      Variable H: history.
-      Variable M: memories.
-      Variable H': SemSB.history.
-      Variable E: SemSB.evolution.
-
-      Hypothesis CoherentMsem: coherent_msem_state H M.
-      Hypothesis CompatEnv: compat_state H M H' E.
-
-      Variable lasts: Env.t const.
-
-      Hypothesis LastsSpec: lasts_spec lasts M.
-
-      (* Fact CompatEnv: *)
-      (*   forall n, *)
-      (*     compat_env (restr_hist H n) lasts (SemSB.restr_hist H' n) (SemSB.restr_evol E n). *)
-      (* Proof. *)
-      (*   now apply compat_hist_spec. *)
-      (* Qed. *)
-      (* Hint Resolve CompatEnv. *)
-
-      Definition correct_clock (ck: clock) (vs: stream value) : Prop :=
-        sem_clock bk H ck (fun n => vs n <>b absent).
-
-      Ltac spe_tac k :=
-        intros until k;
-        let Sem := fresh in
-        let n := fresh in
-        intros Sem ** n; specialize (Sem n); eauto.
-
-      Tactic Notation "spe" integer(k) :=
-        spe_tac k.
-
-      Lemma var_var_correctness:
-        forall x vs,
-          (forall n, find_val x (M n) = None) ->
-          sem_var H x vs ->
-          SemSB.sem_var_var H' x vs.
-      Proof. spe 1. Qed.
-      Hint Resolve var_var_correctness.
-
-      Lemma clock_correctness:
-        forall ck bs,
-          sem_clock bk H ck bs ->
-          SemSB.sem_clock bk H' E (translate_clock lasts ck) bs.
-      Proof. spe 0. Qed.
-      Hint Resolve clock_correctness.
-
-      Lemma state_var_correctness:
-        forall x vs ck,
-          (forall n, find_val x (M n) <> None) ->
-          sem_var H x vs ->
-          correct_clock ck vs ->
-          SemSB.sem_state_var bk H' E (translate_clock lasts ck) x vs.
-      Proof. spe 2. Qed.
-      Hint Resolve state_var_correctness.
-
-      Lemma var_correctness:
-        forall x vs ck,
-          sem_var H x vs ->
-          correct_clock ck vs ->
-          SemSB.sem_var bk H' E (translate_clock lasts ck) (tovar lasts x) vs.
-      Proof. spe 1. Qed.
-      Hint Resolve var_correctness.
-
-      Lemma lexp_correctness:
-        forall e vs ck vars,
-          sem_lexp bk H e vs ->
-          wc_lexp vars e ck ->
-          correct_clock ck vs ->
-          SemSB.sem_lexp bk H' E (translate_clock lasts ck) (translate_lexp lasts e) vs.
-      Proof. spe 2. Qed.
-      Hint Resolve lexp_correctness.
-
-      Lemma cexp_correctness:
-        forall e vs ck vars,
-          sem_cexp bk H e vs ->
-          wc_cexp vars e ck ->
-          correct_clock ck vs ->
-          SemSB.sem_cexp bk H' E (translate_clock lasts ck) (translate_cexp lasts e) vs.
-      Proof. spe 2. Qed.
-      Hint Resolve cexp_correctness.
-
-      Lemma laexp_correctness:
-        forall e ck vs vars,
-          sem_laexp bk H ck e vs ->
-          wc_lexp vars e ck ->
-          SemSB.sem_laexp bk H' E (translate_clock lasts ck) (translate_lexp lasts e) vs.
-      Proof. spe 0. Qed.
-
-      Lemma caexp_correctness:
-        forall e ck vs vars,
-          sem_caexp bk H ck e vs ->
-          wc_cexp vars e ck ->
-          SemSB.sem_caexp bk H' E (translate_clock lasts ck) (translate_cexp lasts e) vs.
-      Proof. spe 0. Qed.
-
-
-    End Sem.
-    Hint Resolve
-         var_var_correctness
-         laexp_correctness
-         caexp_correctness.
-
-    Inductive relooper: Env.t const -> SemSB.evolution -> SemSB.evolution -> Prop :=
-      relooper_intro:
-        forall E E' lasts,
-        (forall x vs vs' c,
-            find_val x E = Some vs ->
-            find_val x E' = Some vs' ->
-            (forall n, vs (S n) = vs' n)
-            /\ vs 0 = sem_const c) ->
-        relooper lasts E E'.
-
-    Inductive coherent_state: SemSB.evolution -> SemSB.transient_evolutions -> SemSB.evolution -> Prop :=
-      coherent_state_intro:
-        forall E T E',
-          (forall x vs,
-              find_val x E = Some vs ->
-              exists vs', find_val x E' = Some vs') ->
-          coherent_state E T E'.
-
-    (* Inductive correspondence: *)
-    (*   history -> Env.t const -> SemSB.history -> SemSB.evolution -> SemSB.transient_evolutions -> SemSB.evolution -> Prop := *)
-    (*   correspondence_intro: *)
-    (*     forall H lasts H' E T E', *)
-    (*       compat_hist H lasts H' E -> *)
-    (*       coherent_state E T E' -> *)
-    (*       relooper lasts E E' -> *)
-    (*       correspondence H lasts H' E T E'. *)
-
-    (* Fact find_mem: *)
-    (*   forall {A} x e (v: A), *)
-    (*     Env.find x e = Some v -> *)
-    (*     Env.mem x e = true. *)
-    (* Proof. *)
-    (*   unfold Env.mem; intros ** ->; auto. *)
-    (* Qed. *)
-    (* Hint Resolve find_mem. *)
-
-    Lemma hold_det:
-      forall v0 xs xs',
-        same_clock (fun n => [xs n; xs' n]) ->
-        hold v0 xs ≈ hold v0 xs' ->
-        xs ≈ xs'.
-    Proof.
-      intros ** Same Eq n.
-      specialize (Eq (S n)); simpl in *.
-      specialize (Same n); destruct Same as [Same|Same].
-      + inversion_clear Same as [|??? Same']; inv Same'; congruence.
-      + inversion_clear Same as [|??? Same']; inv Same'; destruct (xs n), (xs' n); congruence.
-    Qed.
-
-    Lemma hold_det':
-      forall n v0 xs xs',
-        instant_same_clock [xs n; xs' n] ->
-        hold v0 xs (S n) = hold v0 xs' (S n) ->
-        xs n = xs' n.
-    Proof.
-      intros ** Same Eq.
-      simpl in *.
-      destruct Same as [Same|Same].
-      + inversion_clear Same as [|??? Same']; inv Same'; congruence.
-      + inversion_clear Same as [|??? Same']; inv Same'; destruct (xs n), (xs' n); congruence.
-    Qed.
-
-    Inductive lasts_eq_spec (lasts: Env.t const) : equation -> Prop :=
-      | LSdef:
-          forall x ck e,
-            Env.mem x lasts = false ->
-            lasts_eq_spec lasts (EqDef x ck e)
-      | LSapp:
-          forall xs ck f es r,
-            Forall (fun x => Env.mem x lasts = false) xs ->
-            lasts_eq_spec lasts (EqApp xs ck f es r)
-      | LSfby:
-          forall x ck c0 e,
-            Env.find x lasts = Some c0 ->
-            lasts_eq_spec lasts (EqFby x ck c0 e).
-
-    Fact hd_error_Some_hd:
-      forall {A} d (xs: list A) x,
-        hd_error xs = Some x ->
-        hd d xs = x.
-    Proof.
-      destruct xs; simpl; intros; try discriminate.
-      now inv H.
-    Qed.
-
-
-
-      Lemma sem_equation_add_inst:
-        forall M M' x eqs,
-          ~ inst_in_eqs x eqs ->
-          Forall (SemSB.sem_equation P bk H M) eqs ->
-          Forall (SemSB.sem_equation P bk H (add_inst x M' M)) eqs.
-      Proof.
-        intros * Hnd Hsem.
-        induction eqs as [|eq eqs IH]; [now constructor|].
-        apply not_inst_in_eqs_cons in Hnd as [Hnd].
-        apply Forall_cons2 in Hsem as [Hsem Hsems].
-        constructor; auto.
-        induction eq; inv Hsem; eauto using SemSB.sem_equation.
-        - econstructor; eauto.
-          unfold sub_inst.
-          unfold sub_inst; rewrite find_inst_gso; auto.
-          intro; apply Hnd; subst; constructor.
-        - econstructor; eauto.
-          unfold sub_inst; rewrite find_inst_gso; auto.
-          intro; apply Hnd; subst; constructor.
-      Qed.
-
-      Lemma sem_equation_add_val:
-        forall M mv x eqs,
-          ~ defined_in_eqs x eqs ->
-          Forall (SemSB.sem_equation P bk H M) eqs ->
-          Forall (SemSB.sem_equation P bk H (add_val x mv M)) eqs.
-      Proof.
-        intros * Hnd Hsem.
-        induction eqs as [|eq eqs IH]; [now constructor|].
-        apply not_defined_in_eqs_cons in Hnd as [Hnd].
-        apply Forall_cons2 in Hsem as [Hsem Hsems].
-        constructor; auto.
-        induction eq; inv Hsem; eauto using SemSB.sem_equation.
-        econstructor; eauto.
-        apply mfby_add_val; auto.
-        intro; subst; apply Hnd; constructor.
-      Qed.
-
-    End Sem.
-
-    Lemma equation_correctness:
-      forall bk H eqs M eq,
-        (forall f xss oss,
-            sem_node G f xss oss ->
-            exists M, SemSB.sem_block P f M xss oss) ->
-        (forall f r xss oss,
-            sem_reset G f r xss oss ->
-            exists M, SemSB.sem_block P f M xss oss
-                 /\ SemSB.reset_regs r M) ->
-        sem_equation G bk H eq ->
-        compat_eq eq eqs ->
-        Forall (SemSB.sem_equation P bk H M) eqs ->
-        SemSB.well_structured_memories eqs M ->
-        exists M', Forall (SemSB.sem_equation P bk H M') (translate_eqn eq ++ eqs)
-              /\ SemSB.well_structured_memories (translate_eqn eq ++ eqs) M'.
-    Proof.
-      intros ** IHnode IHreset Heq WF Heqs WS.
-      inv Heq; simpl; inv WF.
-      - repeat (econstructor; eauto).
-      - edestruct IHnode as (M' & Block); eauto.
-        exists (add_inst (hd default x) M' M); split.
-        + constructor.
-          * econstructor; eauto.
-            apply find_inst_gss.
-          * apply sem_equation_add_inst; auto.
-        + apply SemSB.well_structured_add_inst_call; auto.
-      - edestruct IHreset as (M' & Block & Reset); eauto.
-        exists (add_inst (hd default x) M' M); split.
-        + constructor.
-          * econstructor; eauto.
-            apply find_inst_gss.
-          *{ constructor.
-             - econstructor; eauto.
-               apply find_inst_gss.
-             - apply sem_equation_add_inst; auto.
-           }
-        + apply SemSB.well_structured_add_inst_reset_call; auto.
-      - exists (add_val x {| SemSB.content := hold (sem_const c0) ls; SemSB.reset := fun _ => false |} M); split.
-        + constructor.
-          *{ econstructor; eauto.
-             econstructor.
-             - apply find_val_gss.
-             - reflexivity.
-             - intro; unfold fby; simpl.
-               destruct (ls n); auto.
-           }
-          * apply sem_equation_add_val; auto.
-        + apply SemSB.well_structured_add_val_fby; auto.
-    Qed.
-
-    Lemma well_structured_empty:
-      SemSB.well_structured_memories [] (empty_memory SemSB.mvalues).
-    Proof.
-      constructor; unfold find_val, find_inst, SemSB.fbys, SemSB.insts;
-        simpl; intros; split; intro H; contradict H; auto; apply not_In_empty.
-    Qed.
-
     Corollary equations_correctness:
-      forall bk H eqs,
-        (forall f xss oss,
-            sem_node G f xss oss ->
-            exists M, SemSB.sem_block P f M xss oss) ->
-        (forall f r xss oss,
-            sem_reset G f r xss oss ->
-            exists M, SemSB.sem_block P f M xss oss
-                 /\ SemSB.reset_regs r M) ->
-        compat_eqs eqs ->
-        Forall (sem_equation G bk H) eqs ->
-        exists M', Forall (SemSB.sem_equation P bk H M') (translate_eqns eqs)
-              /\ SemSB.well_structured_memories (translate_eqns eqs) M'.
+      forall G bk H M M' eqs,
+        (forall f xss M M' yss,
+            msem_node G f xss M M' yss ->
+            sem_block_n (translate G) f M xss yss M') ->
+        Ordered_nodes G ->
+        Forall (msem_equation G bk H M M') eqs ->
+        exists Is, sem_equations_n (translate G) bk H M Is M' (translate_eqns eqs).
     Proof.
-      intros ** IHnode IHreset WF Heqs.
-      induction eqs as [|eq eqs IHeqs].
-      - exists (@empty_memory SemSB.mvalues).
-        split; try now constructor.
-        apply well_structured_empty.
+      intros ** Hord IH Heqs.
+      unfold translate_eqns, concatMap.
+      induction eqs as [|eq eqs IHeqs]; simpl.
+      - exists (fun n => Env.empty state); constructor.
       - apply Forall_cons2 in Heqs as [Heq Heqs].
-        inv WF.
-        eapply IHeqs in Heqs as [? ()]; eauto.
-        unfold translate_eqns; rewrite concatMap_cons.
+        eapply IHeqs in Heqs as (?&?).
         eapply equation_correctness; eauto.
     Qed.
 
-    Lemma find_block_later_not_is_block_in:
-      forall b n bl P',
-        Ordered_nodes (n :: G) ->
-        SynSB.find_block b P = Some (bl, P') ->
-        ~ is_block_in n.(n_name) bl.(SynSB.b_eqs).
+    Lemma clock_of_correctness:
+      forall xss bk,
+        ExprSem.clock_of xss bk ->
+        forall n, clock_of (xss n) (bk n).
+    Proof. auto. Qed.
+
+    Lemma same_clock_correctness:
+      forall xss,
+        ExprSem.same_clock xss ->
+        forall n, same_clock (xss n).
+    Proof. auto. Qed.
+    Hint Resolve clock_of_correctness same_clock_correctness.
+
+    Lemma not_Is_node_in_not_Is_block_in:
+      forall eqs f,
+        ~ Is_node_in f eqs ->
+        ~ Is_block_in f (translate_eqns eqs).
     Proof.
-      intros ** Hord Hfind Hini.
-      pose proof (SynSB.find_block_name _ _ _ _ Hfind) as Hb.
-      apply find_block_translate in Hfind as (n' & Hfind' & E).
-      rewrite E in Hini; simpl in Hini.
-      apply is_block_is_node in Hini.
-      eapply find_node_later_not_Is_node_in; eauto.
+      unfold translate_eqns, concatMap.
+      induction eqs as [|eq]; simpl; intros ** Hnin Hin.
+      - inv Hin.
+      - apply not_Is_node_in_cons in Hnin as (Hnineq & Hnin).
+        apply IHeqs in Hnin.
+        destruct eq; simpl in *.
+        + inversion_clear Hin as [?? E|?? Hins]; try inv E; auto.
+        + destruct o as [[]|]; inversion_clear Hin as [?? E|?? Hins]; auto.
+          * inv E; apply Hnineq; constructor.
+          * inversion_clear Hins as [?? E|?? Hins']; auto.
+            inv E; apply Hnineq; constructor.
+          * inv E; apply Hnineq; constructor.
+        + inversion_clear Hin as [?? E|?? Hins]; try inv E; auto.
     Qed.
 
-    Lemma find_block_not_is_block_in:
-      forall b bl P',
+    Theorem correctness:
+      forall G f xss M M' yss,
         Ordered_nodes G ->
-        SynSB.find_block b P = Some (bl, P') ->
-        ~ is_block_in bl.(SynSB.b_name) bl.(SynSB.b_eqs).
+        msem_node G f xss M M' yss ->
+        sem_block_n (translate G) f M xss yss M'.
     Proof.
-      intros ** Hord Hfind Hini.
-      pose proof (SynSB.find_block_name _ _ _ _ Hfind) as Hb.
-      apply find_block_translate in Hfind as (n' & Hfind' & E).
-      apply find_node_split in Hfind' as [G' [aG Hge]].
-      rewrite Hge in Hord.
-      apply Ordered_nodes_append in Hord.
-      inversion_clear Hord as [|? ? Hord' Heqs Hnin].
-      destruct (Heqs (SynSB.b_name bl)) as (Eq).
-      - subst bl; simpl in *.
-        clear - Hini.
-        induction (n_eqs n') as [|eq]; simpl in *.
-        + inv Hini.
-        + unfold translate_eqns, concatMap, is_block_in in Hini; simpl in Hini.
-          unfold is_block_in in Hini; rewrite Exists_app' in Hini.
-          destruct Hini as [Hini|Hini].
-          * left.
-            destruct eq; try destruct o as [()|]; simpl in Hini;
-              inversion_clear Hini as [?? In|?? Nil];
-              try inversion_clear Nil as [?? In|?? Nil']; try inv In; try inv Nil';
-                constructor.
-          * right. apply IHl; auto.
-      - apply Eq; subst bl; reflexivity.
-    Qed.
-
-    Lemma sem_block_cons:
-      forall n f xs M ys,
-        Ordered_nodes (n :: G) ->
-        n.(n_name) <> f ->
-        SemSB.sem_block (translate (n :: G)) f xs M ys ->
-        SemSB.sem_block P f xs M ys.
-    Proof.
-      intros ** Hord Hnf Hsem.
-      revert Hnf.
-      induction Hsem
-        as [| | | |????????? Hfind ????? Heqs WS IHeqs]
-             using SemSB.sem_block_mult
-        with (P_equation := fun bk H M eq =>
-                              ~ is_block_in_eq n.(n_name) eq ->
-                              SemSB.sem_equation (translate G) bk H M eq);
-        eauto using SemSB.sem_equation.
-      - intros Hnin.
+      induction G as [|node ? IH].
+      inversion 2;
+        match goal with Hf: find_node _ [] = _ |- _ => inversion Hf end.
+      intros ** Hord Hsem n.
+      assert (Hsem' := Hsem).
+      inversion_clear Hsem' as [???????? Clock Hfind Ins Outs ??? Heqs].
+      pose proof (find_node_not_Is_node_in _ _ _ Hord Hfind) as Hnini.
+      pose proof Hord; inversion_clear Hord as [|??? NodeIn].
+      pose proof Hfind as Hfind'.
+      simpl in Hfind.
+      assert (Ordered_blocks (translate_node node :: translate G))
+        by (change (translate_node node :: translate G) with (translate (node :: G));
+            apply Ordered_nodes_blocks; auto).
+      destruct (ident_eqb node.(n_name) f) eqn:Hnf.
+      - inversion Hfind; subst n0.
+        apply find_node_translate in Hfind' as (?&?&?&?); subst.
+        eapply Forall_msem_equation_global_tl in Heqs; eauto.
+        apply equations_correctness in Heqs as (?&Heqs); auto.
         econstructor; eauto.
-        apply IHHsem.
-        intro Hnb; apply Hnin.
-        rewrite Hnb; constructor.
-      - intro; simpl in Hfind; apply ident_eqb_neq in Hnf; rewrite Hnf in Hfind; eauto.
-        econstructor; eauto.
-        assert (Forall (fun eq => ~ is_block_in_eq (n_name n) eq) (SynSB.b_eqs bl)) as NotIns
-            by (eapply is_block_in_Forall, find_block_later_not_is_block_in; eauto).
-        clear Heqs WS.
-        induction (SynSB.b_eqs bl); inv NotIns; inv IHeqs; constructor; auto.
+        + specialize (Ins n); destruct node; simpl in *.
+          rewrite map_fst_idty; eauto.
+        + specialize (Outs n); destruct node; simpl in *.
+          rewrite map_fst_idty; eauto.
+        + apply sem_equations_cons2; eauto.
+          apply not_Is_node_in_not_Is_block_in; auto.
+      - assert (n_name node <> f) by now apply ident_eqb_neq.
+        eapply msem_node_cons, IH in Hsem; eauto.
+        apply sem_block_cons2; auto using Ordered_blocks.
     Qed.
-
-    Lemma sem_block_cons2:
-      forall n f xs M ys,
-        Forall (fun n' => n_name n <> n_name n') G ->
-        SemSB.sem_block P f xs M ys ->
-        SemSB.sem_block (translate (n :: G)) f xs M ys.
-    Proof.
-      intros ** Hnin Hsem.
-      induction Hsem
-        as [| | | |????????? Hfind]
-             using SemSB.sem_block_mult
-        with (P_equation := fun bk H M eq =>
-                              SemSB.sem_equation (translate (n :: G)) bk H M eq);
-        eauto using SemSB.sem_equation.
-      econstructor; eauto.
-      simpl.
-      assert (n.(n_name) <> b) as Hnf.
-      { intro Hnf.
-        rewrite Hnf in *.
-        pose proof (SynSB.find_block_name _ _ _ _ Hfind) as Hb.
-        apply find_block_translate in Hfind as (n' & Hfind' & ?).
-        apply find_node_split in Hfind' as [G' [aG Hge]].
-        rewrite Hge in Hnin.
-        apply Forall_app in Hnin.
-        destruct Hnin as [H' Hfg]; clear H'.
-        inversion_clear Hfg.
-        match goal with H:b<>_ |- False => apply H end.
-        rewrite <-Hb; subst bl; auto.
-      }
-      apply ident_eqb_neq in Hnf; rewrite Hnf.
-      eauto.
-    Qed.
-
-    Lemma sem_equation_cons:
-      forall bk H M eqs n,
-        Ordered_nodes (n :: G) ->
-        ~Is_node_in n.(n_name) eqs ->
-        Forall (SemSB.sem_equation P bk H M) (translate_eqns eqs) ->
-        Forall (SemSB.sem_equation (translate (n :: G)) bk H M) (translate_eqns eqs).
-    Proof.
-      intros ** Hord Hnini Hsem.
-      induction eqs as [|eq eqs IH]; [now constructor|].
-      unfold translate_eqns in *; rewrite concatMap_cons in Hsem.
-      apply Forall_app in Hsem as [Heq Heqs].
-      apply not_Is_node_in_cons in Hnini.
-      destruct Hnini as [Hnini Hninis].
-      apply IH with (1:=Hninis) in Heqs.
-      rewrite concatMap_cons.
-      apply Forall_app; split; auto.
-      inv Hord.
-      induction eq; simpl in *.
-      - constructor; auto.
-        inversion_clear Heq as [|?? Hsem].
-        inv Hsem; eauto using SemSB.sem_equation.
-      - destruct o as [(r, ckr)|]; inversion_clear Heq as [|?? Hsem Heq'];
-          constructor; inv Hsem; econstructor; eauto.
-        + inversion_clear Heq' as [|?? Hsem'].
-          inv Hsem'; econstructor; eauto.
-          apply sem_block_cons2; auto.
-        + apply sem_block_cons2; auto.
-      - constructor; auto.
-        inversion_clear Heq as [|?? Hsem].
-        inv Hsem; eauto using SemSB.sem_equation.
-    Qed.
-
-  End Global.
-
-
-  Fixpoint path_inst (p: list ident) (M: SemSB.memories) : option SemSB.memories :=
-    match p with
-    | [] => Some M
-    | x :: p =>
-      match find_inst x M with
-      | Some M => path_inst p M
-      | None => None
-      end
-    end.
-
-  Lemma path_inst_last:
-    forall p M M' x M'',
-      path_inst p M = Some M' ->
-      sub_inst x M' M'' ->
-      path_inst (p ++ [x]) M = Some M''.
-  Proof.
-    induction p as [|y]; simpl; intros ** Path Sub.
-    - inv Path; rewrite Sub; auto.
-    - destruct (find_inst y M); inv Path; eauto.
-  Qed.
-
-  Section Choices.
-
-    Variable Fm: nat -> SemSB.memories.
-    Variable Fh: nat -> history.
-    Variable Fmvs: nat -> SemSB.mvalues.
-    Variable r: stream bool.
-
-    Definition reset_content (x: ident) (p: list ident) : stream val :=
-      fun n => match path_inst p (Fm (count r n)) with
-            | Some M =>
-              match find_val x M with
-              | Some mv => mv.(SemSB.content) n
-              | None => false_val
-              end
-            | None => false_val
-            end.
-
-    Definition reset_reset (x: ident) (p: list ident) : stream bool :=
-      fun n => match path_inst p (Fm (count r n)) with
-            | Some M =>
-              match find_val x M with
-              | Some mv => r n || mv.(SemSB.reset) n
-              | None => r n
-              end
-            | None => r n
-            end.
-
-    Lemma reset_reset_spec:
-      forall n x p,
-        r n = true ->
-        reset_reset x p n = true.
-    Proof.
-      unfold reset_reset; intros ** ->.
-      destruct (path_inst p (Fm (count r n))); auto.
-      destruct (find_val x m); auto.
-    Qed.
-
-    Definition reset_memories_path (p: list ident) (M0: SemSB.memories) : SemSB.memories :=
-      mmapi (fun p x mv =>
-               {| SemSB.content := reset_content x p;
-                  SemSB.reset := reset_reset x p |})
-            p M0.
-
-    Definition reset_memories := reset_memories_path [].
-
-    Lemma sub_inst_reset_memories_path:
-      forall x p M M',
-        sub_inst x M M' ->
-        sub_inst x (reset_memories_path p M) (reset_memories_path (p ++ [x]) M').
-    Proof.
-      intros ** Find; unfold sub_inst, reset_memories_path.
-      rewrite find_inst_mmapi, Find; auto.
-    Qed.
-
-    Lemma sub_inst_reset_memories_path':
-      forall x p M M',
-        sub_inst x (reset_memories_path p M) M' ->
-        exists M'', M' = reset_memories_path (p ++ [x]) M''
-               /\ sub_inst x M M''.
-    Proof.
-      unfold sub_inst, reset_memories_path; intros ** Find.
-      rewrite find_inst_mmapi in Find.
-      destruct (find_inst x M) eqn: E; inv Find; eauto.
-    Qed.
-
-    Lemma reset_memories_path_spec:
-      forall k p r',
-        (forall n,
-            r' n = true ->
-            r n = true) ->
-        SemSB.reset_regs r' (reset_memories_path p (Fm k)).
-    Proof.
-      intros ** Spec; unfold reset_memories_path.
-      revert p.
-      induction (Fm k) as [?? IH] using memory_ind'.
-      constructor.
-      - intros x mvs.
-        unfold find_val.
-        simpl; rewrite Env.find_mapi.
-        intro Find.
-        destruct (Env.find x xvs); inv Find; auto.
-        intros; simpl; apply reset_reset_spec; auto.
-      - induction xms as [|[y]].
-        + intros; discriminate.
-        + simpl in IH; inv IH.
-          intros x M'.
-          unfold sub_inst, find_inst.
-          simpl.
-          destruct (Env.POTB.compare x y); simpl;
-            intro Find; inv Find; eauto.
-    Qed.
-
-    Corollary reset_memories_path_sub_spec:
-      forall k p r' x M,
-        sub_inst x (Fm k) M ->
-        (forall n, r' n = true -> r n = true) ->
-        SemSB.reset_regs r' (reset_memories_path (p ++ [x]) M).
-    Proof.
-      intros ** Sub Spec; eapply reset_memories_path_spec with (k := k) in Spec.
-      inversion_clear Spec as [??? Inst]; eapply Inst, sub_inst_reset_memories_path; eauto.
-    Qed.
-
-    Corollary reset_memories_spec:
-      forall k r',
-        (forall n, r' n = true -> r n = true) ->
-        SemSB.reset_regs r (reset_memories (Fm k)).
-    Proof.
-      intros; now apply reset_memories_path_spec.
-    Qed.
-
-    Definition reset_history (H0: history) : history :=
-      PM.mapi (fun x _ => fun n => match PM.find x (Fh (count r n)) with
-                             | Some xs => xs n
-                             | None => absent
-                             end) H0.
-
-    Definition reset_mvalues: SemSB.mvalues :=
-    {| SemSB.content := fun n => (Fmvs (count r n)).(SemSB.content) n;
-       SemSB.reset := fun n => r n || (Fmvs (count r n)).(SemSB.reset) n |}.
-
-    Lemma reset_mvalues_spec:
-      forall x e c0 ck xss,
-        (forall n, 0 < length (xss n)) ->
-        (forall k,
-            exists bk xs ls,
-              sem_var (Fh k) x xs
-              /\ sem_laexp bk (Fh k) ck e ls
-              /\ find_val x (Fm k) = Some (Fmvs k)
-              /\ SemSB.content (Fmvs k) 0 = sem_const c0
-              /\ (forall n : nat,
-                    match ls n with
-                    | absent =>
-                      SemSB.content (Fmvs k) (S n) =
-                      (if SemSB.reset (Fmvs k) (S n)
-                       then sem_const c0
-                       else SemSB.content (Fmvs k) n)
-                      /\ xs n = absent
-                    | present v' =>
-                      SemSB.content (Fmvs k) (S n) =
-                      (if SemSB.reset (Fmvs k) (S n)
-                       then sem_const c0
-                       else v')
-                      /\ xs n = present (SemSB.content (Fmvs k) n)
-                    end)
-              /\ clock_of (mask (all_absent (xss 0)) k r xss) bk) ->
-        forall n, r n = true ->
-             SemSB.content reset_mvalues n = sem_const c0.
-    Proof.
-      intros ** Length Spec n E.
-      unfold reset_mvalues; simpl.
-      induction n; simpl; rewrite E.
-      - destruct (Spec 1) as (?&?&?&?); intuition.
-      - specialize (Spec (S (count r n))); destruct Spec as (bk &?&?&?& Hexp &?& Init & Heq & Clock).
-        assert (forall n',
-                   n' <= n ->
-                   interp_laexp_instant (bk n') (restr_hist (Fh (S (count r n))) n') ck e = absent)
-          as Absent.
-        { assert (forall n',
-                     n' <= n ->
-                     bk n' = false) as Hbk.
-          { clear - Clock Length.
-            intros ** Lte.
-            specialize (Clock n').
-            rewrite mask_opaque in Clock; auto.
-            - apply Bool.not_true_is_false; intro Ebk.
-              apply Clock in Ebk.
-              specialize (Length 0).
-              clear - Ebk Length; induction (xss 0); simpl in *; inv Ebk; auto; omega.
-            - apply Lt.le_lt_or_eq in Lte as [Lt|]; subst; auto.
-              apply (count_le' r) in Lt; omega.
-          }
-          intros.
-          specialize (Hexp n'); simpl in Hexp.
-          pose proof Hexp as Hexp'; apply interp_laexp_instant_sound in Hexp'; rewrite Hexp' in Hexp.
-          destruct (interp_laexp_instant (bk n') (restr_hist (Fh (S (count r n))) n') ck e); auto.
-          inversion_clear Hexp as [???? HClock|].
-          rewrite Hbk in HClock; auto; contradict HClock.
-          apply not_subrate_clock.
-        }
-        assert (forall n', n' <= n -> SemSB.content (Fmvs (S (count r n))) n' = sem_const c0) as Spec.
-        { intros ** Lte.
-          induction n'; auto.
-          specialize (Hexp n'); simpl in Hexp; apply interp_laexp_instant_sound in Hexp.
-          specialize (Heq n').
-          rewrite Hexp, Absent in Heq; try omega; destruct Heq as (->).
-          destruct (SemSB.reset (Fmvs (S (count r n))) (S n')); auto.
-          apply IHn'; omega.
-        }
-        specialize (Hexp n); simpl in Hexp; apply interp_laexp_instant_sound in Hexp.
-        specialize (Heq n);
-          rewrite Hexp, Absent in Heq; auto; destruct Heq as (->).
-        destruct (SemSB.reset (Fmvs (S (count r n))) (S n)); auto.
-    Qed.
-
-    Lemma find_val_reset_memories:
-      forall x,
-        (forall k, find_val x (Fm k) = Some (Fmvs k)) ->
-        find_val x (reset_memories (Fm 0)) = Some reset_mvalues.
-    Proof.
-      intros ** Spec.
-      unfold reset_mvalues, reset_memories, reset_memories_path.
-      rewrite find_val_mmapi.
-      destruct (find_val x (Fm 0)) eqn: E; simpl.
-      - do 3 f_equal.
-        + unfold reset_content; simpl.
-          extensionality n.
-          rewrite Spec; auto.
-        + unfold reset_reset.
-          extensionality n.
-          simpl; rewrite Spec; auto.
-      - rewrite Spec in E; discriminate.
-    Qed.
-
-    Section InterpReset.
-
-      Variable n: nat.
-
-      Definition spec_var (x: ident) : Prop :=
-        forall k, PM.find x (Fh k) <> None.
-
-      Definition spec_vars := Forall spec_var.
-
-      Inductive spec_clock: clock -> Prop :=
-      | spec_clock_base:
-          spec_clock Cbase
-      | spec_clock_con:
-          forall ck x b,
-            spec_var x ->
-            spec_clock ck ->
-            spec_clock (Con ck x b).
-
-      Inductive spec_lexp: lexp -> Prop :=
-      | spec_lexp_const:
-          forall c,
-            spec_lexp (Econst c)
-      | spec_lexp_var:
-          forall x t,
-            spec_var x ->
-            spec_lexp (Evar x t)
-      | spec_lexp_when:
-          forall e x b,
-            spec_var x ->
-            spec_lexp e ->
-            spec_lexp (Ewhen e x b)
-      | spec_lexp_unop:
-          forall op e t,
-            spec_lexp e ->
-            spec_lexp (Eunop op e t)
-      | spec_lexp_binop:
-          forall op e1 e2 t,
-            spec_lexp e1 ->
-            spec_lexp e2 ->
-            spec_lexp (Ebinop op e1 e2 t).
-
-      Definition spec_lexps := Forall spec_lexp.
-
-      Inductive spec_cexp: cexp -> Prop :=
-      | spec_cexp_merge:
-          forall x e1 e2,
-            spec_var x ->
-            spec_cexp e1 ->
-            spec_cexp e2 ->
-            spec_cexp (Emerge x e1 e2)
-      | spec_cexp_ite:
-          forall le e1 e2,
-            spec_lexp le ->
-            spec_cexp e1 ->
-            spec_cexp e2 ->
-            spec_cexp (Eite le e1 e2)
-      | spec_cexp_exp:
-          forall e,
-            spec_lexp e ->
-            spec_cexp (Eexp e).
-
-      Inductive spec_eq: SynSB.equation -> Prop :=
-      | spec_eq_def:
-          forall x ck e,
-            spec_var x ->
-            spec_clock ck ->
-            spec_cexp e ->
-            spec_eq (SynSB.EqDef x ck e)
-      | spec_eq_fby:
-          forall x ck c0 e,
-            spec_var x ->
-            spec_clock ck ->
-            spec_lexp e ->
-            spec_eq (SynSB.EqFby x ck c0 e)
-      | spec_eq_reset:
-          forall ck b i r,
-            spec_var r ->
-            spec_eq (SynSB.EqReset ck b i r)
-      | spec_eq_call:
-          forall xs ck b i es,
-            spec_vars xs ->
-            spec_clock ck ->
-            spec_lexps es ->
-            spec_eq (SynSB.EqCall xs ck b i es).
-
-      Lemma sem_var_instant_reset:
-        forall x v,
-          spec_var x ->
-          sem_var_instant (restr_hist (Fh (count r n)) n) x v ->
-          sem_var_instant (restr_hist (reset_history (Fh 0)) n) x v.
-      Proof.
-        intros ** Spec Sem.
-        induction Sem; constructor.
-        unfold reset_history, restr_hist, PM.map in *.
-        repeat rewrite PM.gmapi in *; rewrite option_map_map.
-        destruct (PM.find x (Fh (count r n))) eqn: E.
-        - destruct (PM.find x (Fh 0)) eqn: E'; auto.
-          exfalso; eapply Spec; eauto.
-        - exfalso; eapply Spec; eauto.
-      Qed.
-      Hint Resolve sem_var_instant_reset.
-
-      Lemma sem_vars_instant_reset:
-        forall xs vs,
-          spec_vars xs ->
-          sem_vars_instant (restr_hist (Fh (count r n)) n) xs vs ->
-          sem_vars_instant (restr_hist (reset_history (Fh 0)) n) xs vs.
-      Proof.
-        intros ** Spec Sem.
-        induction Sem; inv Spec; constructor; auto.
-        apply IHSem; auto.
-      Qed.
-
-      Variable bk: stream bool.
-      Variable xss: stream (list value).
-      Hypothesis Clk: clock_of (mask (all_absent (xss 0)) (count r n) r xss) bk.
-      Let bk' := clock_of' xss.
-
-      Lemma sem_clock_instant_reset:
-        forall ck b,
-          spec_clock ck ->
-          sem_clock_instant (bk n) (restr_hist (Fh (count r n)) n) ck b ->
-          sem_clock_instant (bk' n) (restr_hist (reset_history (Fh 0)) n) ck b.
-      Proof.
-        intros ** Spec Sem; induction Sem; inv Spec; eauto using sem_clock_instant.
-        apply clock_of_equiv' in Clk; rewrite Clk.
-        subst bk'.
-        unfold clock_of'.
-        rewrite mask_transparent; constructor.
-      Qed.
-      Hint Resolve sem_clock_instant_reset.
-
-      Lemma sem_lexp_instant_reset:
-        forall e v,
-          spec_lexp e ->
-          sem_lexp_instant (bk n) (restr_hist (Fh (count r n)) n) e v ->
-          sem_lexp_instant (bk' n) (restr_hist (reset_history (Fh 0)) n) e v.
-      Proof.
-        intros ** Spec Sem; induction Sem; inv Spec; eauto using sem_lexp_instant.
-        constructor; subst.
-        apply clock_of_equiv' in Clk; rewrite Clk.
-        unfold clock_of'.
-        rewrite mask_transparent; auto.
-      Qed.
-      Hint Resolve sem_lexp_instant_reset.
-
-      Lemma sem_lexps_instant_reset:
-        forall es vs,
-          spec_lexps es ->
-          sem_lexps_instant (bk n) (restr_hist (Fh (count r n)) n) es vs ->
-          sem_lexps_instant (bk' n) (restr_hist (reset_history (Fh 0)) n) es vs.
-      Proof.
-        unfold sem_lexps_instant; intros ** Spec Sem;
-          induction Sem; inv Spec; constructor; eauto.
-      Qed.
-      Hint Resolve sem_lexps_instant_reset.
-
-      Lemma sem_laexp_instant_reset:
-        forall ck e v,
-          spec_clock ck ->
-          spec_lexp e ->
-          sem_laexp_instant (bk n) (restr_hist (Fh (count r n)) n) ck e v ->
-          sem_laexp_instant (bk' n) (restr_hist (reset_history (Fh 0)) n) ck e v.
-      Proof.
-        induction 3; constructor; auto.
-      Qed.
-
-      Lemma sem_laexps_instant_reset:
-        forall ck es vs,
-          spec_clock ck ->
-          spec_lexps es ->
-          sem_laexps_instant (bk n) (restr_hist (Fh (count r n)) n) ck es vs ->
-          sem_laexps_instant (bk' n) (restr_hist (reset_history (Fh 0)) n) ck es vs.
-      Proof.
-        induction 3.
-        - eapply SLticks; eauto.
-        - apply SLabss; auto.
-      Qed.
-
-      Lemma sem_cexp_instant_reset:
-        forall e v,
-          spec_cexp e ->
-          sem_cexp_instant (bk n) (restr_hist (Fh (count r n)) n) e v ->
-          sem_cexp_instant (bk' n) (restr_hist (reset_history (Fh 0)) n) e v.
-      Proof.
-        intros ** Spec Sem; induction Sem; inv Spec; eauto using sem_cexp_instant.
-      Qed.
-      Hint Resolve sem_cexp_instant_reset.
-
-      Lemma sem_caexp_instant_reset:
-        forall ck e v,
-          spec_clock ck ->
-          spec_cexp e ->
-          sem_caexp_instant (bk n) (restr_hist (Fh (count r n)) n) ck e v ->
-          sem_caexp_instant (bk' n) (restr_hist (reset_history (Fh 0)) n) ck e v.
-      Proof.
-        induction 3; constructor; auto.
-      Qed.
-
-    End InterpReset.
-
-    Lemma sem_spec_var_instant:
-      forall x,
-        (forall k n, exists v, sem_var_instant (restr_hist (Fh k) n) x v) ->
-        spec_var x.
-    Proof.
-      intros ** Sem k E; destruct (Sem k 0) as (?& Sem');
-        inversion_clear Sem' as [?? Find].
-      unfold restr_hist, PM.map in Find.
-      rewrite PM.gmapi, E in Find.
-      discriminate.
-    Qed.
-
-    Corollary sem_spec_var:
-      forall x,
-        (forall k, exists xs, sem_var (Fh k) x xs) ->
-        spec_var x.
-    Proof.
-      intros x Sem; apply sem_spec_var_instant.
-      intros; destruct (Sem k) as (?& Sem');
-        specialize (Sem' n); eauto.
-    Qed.
-
-    Lemma sem_spec_vars_instant:
-      forall xs,
-        (forall k n, exists xss, sem_vars_instant (restr_hist (Fh k) n) xs xss) ->
-        spec_vars xs.
-    Proof.
-      intros ** Sem; induction xs; constructor.
-      - apply sem_spec_var_instant; intros; destruct (Sem k n) as (?& Sem'); inv Sem'; eauto.
-      - apply IHxs; intros; destruct (Sem k n) as (?& Sem'); inv Sem'; eauto.
-    Qed.
-
-    Corollary sem_spec_vars:
-      forall xs,
-        (forall k, exists xss, sem_vars (Fh k) xs xss) ->
-        spec_vars xs.
-    Proof.
-      intros ** Sem; apply sem_spec_vars_instant.
-      intros; destruct (Sem k) as (?& Sem'); specialize (Sem' n); eauto.
-    Qed.
-
-    Lemma sem_spec_clock_instant:
-      forall ck,
-        (forall k n, exists base b, sem_clock_instant base (restr_hist (Fh k) n) ck b) ->
-        spec_clock ck.
-    Proof.
-      intros ** Sem; induction ck; constructor.
-      - apply sem_spec_var_instant; intros.
-        destruct (Sem k n) as (?&?& Clock); inv Clock; eauto.
-      - apply IHck.
-        intros; destruct (Sem k n) as (?&?& Clock); inv Clock; eauto.
-    Qed.
-
-    Corollary sem_spec_clock_caexp:
-      forall ck e,
-        (forall k, exists bk vs, sem_caexp bk (Fh k) ck e vs) ->
-        spec_clock ck.
-    Proof.
-      intros ** Sem; apply sem_spec_clock_instant.
-      intros; destruct (Sem k) as (?&?& Sem'); specialize (Sem' n); simpl in Sem'.
-      inv Sem'; eauto.
-    Qed.
-
-    Corollary sem_spec_clock_laexp:
-      forall ck e,
-        (forall k, exists bk vs, sem_laexp bk (Fh k) ck e vs) ->
-        spec_clock ck.
-    Proof.
-      intros ** Sem; apply sem_spec_clock_instant.
-      intros; destruct (Sem k) as (?&?& Sem'); specialize (Sem' n); simpl in Sem'.
-      inv Sem'; eauto.
-    Qed.
-
-    Lemma sem_spec_clock_laexps:
-      forall ck es,
-        (forall k, exists bk vss, sem_laexps bk (Fh k) ck es vss) ->
-        spec_clock ck.
-    Proof.
-      intros ** Sem; apply sem_spec_clock_instant.
-      intros; destruct (Sem k) as (?&?& Sem'); specialize (Sem' n); simpl in Sem'.
-      inv Sem'; eauto.
-    Qed.
-
-    Lemma sem_spec_lexp_instant:
-      forall e,
-        (forall k n, exists base v, sem_lexp_instant base (restr_hist (Fh k) n) e v) ->
-        spec_lexp e.
-    Proof.
-      intros ** Sem; induction e; auto using spec_lexp.
-      - constructor; apply sem_spec_var_instant;
-          intros; destruct (Sem k n) as (?&?& Sem'); inv Sem'; eauto.
-      - constructor.
-        + apply sem_spec_var_instant; intros; destruct (Sem k n) as (?&?& Sem'); inv Sem'; eauto.
-        + apply IHe; intros; destruct (Sem k n) as (?&?& Sem'); inv Sem'; eauto.
-      - constructor; apply IHe; intros; destruct (Sem k n) as (?&?& Sem'); inv Sem'; eauto.
-      - constructor.
-        + apply IHe1; intros; destruct (Sem k n) as (?&?& Sem'); inv Sem'; eauto.
-        + apply IHe2; intros; destruct (Sem k n) as (?&?& Sem'); inv Sem'; eauto.
-    Qed.
-
-    Corollary sem_spec_laexp:
-      forall e ck,
-        (forall k, exists bk vs, sem_laexp bk (Fh k) ck e vs) ->
-        spec_lexp e.
-    Proof.
-      intros ** Sem.
-      apply sem_spec_lexp_instant; intros.
-      destruct (Sem k) as (?&?& Sem'); specialize (Sem' n); inv Sem'; eauto.
-    Qed.
-
-    Lemma sem_spec_cexp_instant:
-      forall e,
-        (forall k n, exists base v, sem_cexp_instant base (restr_hist (Fh k) n) e v) ->
-        spec_cexp e.
-    Proof.
-      intros ** Sem; induction e.
-      - constructor.
-        + apply sem_spec_var_instant; intros; destruct (Sem k n) as (?&?& Sem'); inv Sem'; eauto.
-        + apply IHe1; intros; destruct (Sem k n) as (?&?& Sem'); inv Sem'; eauto.
-        + apply IHe2; intros; destruct (Sem k n) as (?&?& Sem'); inv Sem'; eauto.
-      - constructor.
-        + apply sem_spec_lexp_instant; intros; destruct (Sem k n) as (?&?& Sem'); inv Sem'; eauto.
-        + apply IHe1; intros; destruct (Sem k n) as (?&?& Sem'); inv Sem'; eauto.
-        + apply IHe2; intros; destruct (Sem k n) as (?&?& Sem'); inv Sem'; eauto.
-      - constructor; apply sem_spec_lexp_instant; intros; destruct (Sem k n) as (?&?& Sem'); inv Sem'; eauto.
-    Qed.
-
-    Corollary sem_spec_caexp:
-      forall e ck,
-        (forall k, exists bk vs, sem_caexp bk (Fh k) ck e vs) ->
-        spec_cexp e.
-    Proof.
-      intros ** Sem.
-      apply sem_spec_cexp_instant; intros.
-      destruct (Sem k) as (?&?& Sem'); specialize (Sem' n); inv Sem'; eauto.
-    Qed.
-
-    Lemma sem_spec_lexps_instant:
-      forall es,
-        (forall k n, exists base vs, sem_lexps_instant base (restr_hist (Fh k) n) es vs) ->
-        spec_lexps es.
-    Proof.
-      intros ** Sem; induction es; constructor.
-      - apply sem_spec_lexp_instant; intros; destruct (Sem k n) as (?&?& Sem'); inv Sem'; eauto.
-      - apply IHes; intros; destruct (Sem k n) as (?&?& Sem'); inv Sem'; eauto.
-    Qed.
-
-    Corollary sem_spec_laexps:
-      forall es ck,
-        (forall k, exists bk vss, sem_laexps bk (Fh k) ck es vss) ->
-        spec_lexps es.
-    Proof.
-      intros ** Sem.
-      apply sem_spec_lexps_instant; intros; destruct (Sem k) as (?&?& Sem'); specialize (Sem' n); inv Sem'; eauto.
-    Qed.
-
-    Ltac sem_spec H :=
-      let k := fresh in
-      let H' := fresh in
-      match goal with
-      | |- spec_var _ => apply sem_spec_var
-      | |- spec_vars _ => apply sem_spec_vars
-      | _: cexp |- spec_clock _ => eapply sem_spec_clock_caexp
-      | _: lexp |- spec_clock _ => eapply sem_spec_clock_laexp
-      | _: list lexp |- spec_clock _ => eapply sem_spec_clock_laexps
-      | |- spec_cexp _ => eapply sem_spec_caexp
-      | |- spec_lexp _ => eapply sem_spec_laexp
-      | |- spec_lexps _ => eapply sem_spec_laexps
-      end;
-      try (intro k; destruct (H k) as (?&?& H'); inv H'; eauto).
-
-    Lemma sem_spec_eq:
-      forall P eq,
-        (forall k, exists bk M, SemSB.sem_equation P bk (Fh k) M eq) ->
-        spec_eq eq.
-    Proof.
-      intros ** Sem; destruct eq;  constructor (sem_spec Sem).
-    Qed.
-
-  End Choices.
-  Hint Resolve reset_memories_spec sub_inst_reset_memories_path.
-
-  Inductive reset_regs_instant (n: nat): bool -> SemSB.memories -> Prop :=
-    reset_regs_instant_intro:
-      forall M b,
-        (forall x mvs,
-            find_val x M = Some mvs ->
-            b = true -> mvs.(SemSB.reset) n = true) ->
-        (forall x M',
-            sub_inst x M M' ->
-            reset_regs_instant n b M') ->
-        reset_regs_instant n b M.
-
-  Lemma sub_inst_reset_regs_instant:
-    forall bs M x M',
-      (forall n, reset_regs_instant n (bs n) M) ->
-      sub_inst x M M' ->
-      forall n, reset_regs_instant n (bs n) M'.
-  Proof.
-    intros ** Rst Sub n.
-    revert dependent M'; revert x.
-    specialize (Rst n); induction Rst as [??? Inst IH].
-    constructor.
-    - intros; apply Inst in Sub.
-      inv Sub; eauto.
-    - intros; eapply IH; eauto.
-  Qed.
-
-  Lemma reset_regs_instant_spec:
-    forall bs M,
-      SemSB.reset_regs bs M <->
-      forall n, reset_regs_instant n (bs n) M.
-  Proof.
-    split.
-    - induction 1 as [?? Val ? IH]; intro; constructor.
-      + intros; eapply Val; eauto.
-      + intros; eapply IH; eauto.
-    - induction M as [?? IH] using memory_ind'; intros Rst; constructor.
-      + intros; specialize (Rst n); inv Rst; eauto.
-      + intros ** Sub; pose proof Sub as Sub'.
-        unfold sub_inst, find_inst in Sub.
-        eapply Env.find_in, in_map with (f := snd) in Sub; simpl in Sub.
-        eapply In_Forall in IH; eauto.
-        apply IH.
-        eapply sub_inst_reset_regs_instant; eauto.
-  Qed.
-
-  Corollary reset_regs_instant_spec':
-    forall bs M n,
-      SemSB.reset_regs bs M ->
-      reset_regs_instant n (bs n) M.
-  Proof.
-    intros ** Rst.
-    rewrite reset_regs_instant_spec in Rst; auto.
-  Qed.
-
-  Inductive same_skeleton: SemSB.memories -> SemSB.memories -> Prop :=
-    same_skeleton_intro:
-      forall M M',
-        (forall x, find_val x M <> None -> find_val x M' <> None) ->
-        (forall x M1,
-            find_inst x M = Some M1 ->
-            exists M2, find_inst x M' = Some M2
-                  /\ same_skeleton M1 M2) ->
-        same_skeleton M M'.
-
-  Lemma same_skeleton_sub_inst:
-    forall M M' x Mx Mx',
-      same_skeleton M M' ->
-      sub_inst x M Mx ->
-      sub_inst x M' Mx' ->
-      same_skeleton Mx Mx'.
-  Proof.
-    inversion_clear 1 as [??? Inst]; intros ** Sub Sub'.
-    apply Inst in Sub as (? & Sub'' & ?).
-    rewrite Sub' in Sub''; inv Sub''; auto.
-  Qed.
-
-  Lemma reset_memories_path_spec_instant':
-    forall r Fm p r' M0 n M',
-      same_skeleton M0 M' ->
-      path_inst p (Fm (count r n)) = Some M' ->
-      reset_regs_instant n r' M' ->
-      reset_regs_instant n r' (reset_memories_path Fm r p M0).
-  Proof.
-    intros ** Same Sub RstSpec.
-    inversion_clear Same as [?? FindVal FindInst].
-
-    revert dependent p.
-    revert dependent M'.
-    induction M0 as [?? IH] using memory_ind'; intros.
-    inversion_clear RstSpec as [?? Val Inst].
-    constructor.
-    - unfold reset_memories_path; intros y mvs Find' Rst; subst.
-      rewrite find_val_mmapi in Find'.
-      destruct (find_val y (Mnode xvs xms)) eqn: E; inv Find'.
-      unfold reset_reset; simpl.
-      rewrite Sub.
-      destruct (find_val y M') eqn: E'.
-      + erewrite Val; eauto 1.
-        apply Bool.orb_true_r.
-      + contradict E'; eapply FindVal; eauto;
-          rewrite E; intro; discriminate.
-    - intros ** Find.
-      apply sub_inst_reset_memories_path' in Find as (M0' &?& Find); subst.
-      unfold sub_inst in Find.
-      pose proof Find as Find'.
-      unfold sub_inst, find_inst in Find.
-      apply Env.find_in, in_map with (f := snd) in Find; simpl in Find.
-      eapply In_Forall in IH; eauto.
-      assert (exists M'', find_inst x M' = Some M''
-                     /\ same_skeleton M0' M'') as (M'' &?& Same)
-          by (apply FindInst in Find' as (?&?&?); eauto).
-      inv Same.
-      eapply IH; eauto.
-      eapply path_inst_last; eauto.
-  Qed.
-
-  Corollary reset_memories_path_sub_spec_instant':
-    forall r Fm x r' M0 n M',
-      same_skeleton M0 M' ->
-      sub_inst x (Fm (count r n)) M' ->
-      reset_regs_instant n r' M' ->
-      reset_regs_instant n r' (reset_memories_path Fm r [x] M0).
-  Proof.
-    intros ** Same Sub RstSpec.
-    eapply reset_memories_path_spec_instant'; eauto.
-    simpl; rewrite Sub; auto.
-  Qed.
-
-  Lemma sem_var_instant_bl_vars:
-    forall xs xs' xss Fh r n,
-      (forall x k n,
-          In x xs' ->
-          exists v, PM.find x (restr_hist (Fh k) n) = Some v) ->
-      incl xs xs' ->
-      sem_vars (Fh (count r n)) xs (mask (all_absent (xss 0)) (count r n) r xss) ->
-      Forall2 (sem_var_instant (restr_hist (reset_history Fh r (Fh 0)) n)) xs (xss n).
-  Proof.
-    intros ** SameDomFh Incl Sem.
-    unfold mask in Sem; specialize (Sem n); simpl in *.
-    rewrite <-EqNat.beq_nat_refl in Sem.
-    induction Sem as [|x ??? Sem]; constructor; auto.
-    - clear IHSem.
-      inversion_clear Sem as [?? Find]; constructor.
-      assert (exists v, PM.find x (restr_hist (Fh 0) n) = Some v)
-        as (? & Find') by (apply SameDomFh, Incl; constructor; auto).
-      unfold restr_hist, reset_history, PM.map in *.
-      repeat rewrite PM.gmapi in *; rewrite option_map_map.
-      destruct (PM.find x (Fh (count r n))); try discriminate.
-      destruct (PM.find x (Fh 0)); try discriminate; auto.
-    - apply IHSem; intros x' **.
-      apply Incl; right; auto.
-  Qed.
-
-  Lemma sem_laexps_interp_mask:
-    forall xss r Fh ck es k bk' ess,
-      let H := reset_history Fh r (Fh 0) in
-      let bk := clock_of' xss in
-      spec_clock Fh ck ->
-      spec_lexps Fh es ->
-      (forall n, 0 < length (xss n)) ->
-      clock_of (mask (all_absent (xss 0)) k r xss) bk' ->
-      sem_laexps bk' (Fh k) ck es ess ->
-      ess ≈ mask (all_absent (interp_laexps bk H ck es 0)) k r (interp_laexps bk H ck es).
-  Proof.
-    intros ** Length Clock Exps n.
-    specialize (Exps n); simpl in Exps.
-    destruct (EqNat.beq_nat k (count r n)) eqn: E.
-    - apply EqNat.beq_nat_true in E; subst k.
-      rewrite mask_transparent; auto.
-      eapply interp_laexps_instant_sound, sem_laexps_instant_reset; eauto.
-    - apply EqNat.beq_nat_false in E.
-      specialize (Clock n).
-      rewrite mask_opaque; rewrite mask_opaque in Clock; auto.
-      inversion_clear Exps as [?????? SemCk|??? Eq].
-      + assert (bk' n = false) as Hbk'.
-        { apply Bool.not_true_is_false; intro Eq.
-          apply Clock in Eq.
-          specialize (Length 0); induction (xss 0); simpl in *; inv Eq; auto; omega.
-        }
-        rewrite Hbk' in *.
-        contradict SemCk; apply not_subrate_clock.
-      + rewrite Eq.
-        unfold interp_laexps, lift, interp_laexps_instant.
-        destruct (forallb (fun v : value => v ==b absent) (interp_lexps_instant (bk 0) (restr_hist H 0) es)
-                          && negb (interp_clock_instant (bk 0) (restr_hist H 0) ck)
-                  || forallb (fun v : value => v <>b absent) (interp_lexps_instant (bk 0) (restr_hist H 0) es)
-                            && interp_clock_instant (bk 0) (restr_hist H 0) ck);
-          unfold interp_lexps_instant; rewrite all_absent_map; auto.
-        unfold all_absent at 3; rewrite all_absent_map; auto.
-  Qed.
-
-  Lemma sem_vars_interp_mask:
-    forall r Fh xs k ess oss oss0,
-      let H := reset_history Fh r (Fh 0) in
-      sem_vars (Fh k) xs oss ->
-      sem_vars (Fh 0) xs oss0 ->
-      (forall n, absent_list (ess n) <-> absent_list (oss n)) ->
-      (forall n, k <> count r n -> absent_list (oss n)) ->
-      oss ≈ mask (all_absent (interp_vars H xs 0)) k r (interp_vars H xs).
-  Proof.
-    intros ** Vars Vars0 Same Abs n.
-    specialize (Vars n); specialize (Vars0 n);
-      specialize (Same n); (* specialize (Eess n) *) simpl in *.
-    unfold mask in *.
-    destruct (EqNat.beq_nat k (count r n)) eqn: E; simpl.
-    - clear Same.
-      revert Vars0; generalize (oss0 n).
-      induction Vars as [|???? Var]; intros; inversion_clear Vars0 as [|???? Var0]; simpl; auto.
-      f_equal; eauto.
-      inversion_clear Var0 as [?? Find0]; inversion_clear Var as [?? Find].
-      unfold interp_var_instant.
-      subst H; unfold reset_history; unfold restr_hist, PM.map in *.
-      rewrite 2 PM.gmapi; simpl.
-      rewrite PM.gmapi in Find0.
-      destruct (PM.find x (Fh 0)); inv Find0; simpl.
-      rewrite PM.gmapi in Find.
-      apply EqNat.beq_nat_true in E; subst k.
-      destruct (PM.find x (Fh (count r n))); inv Find; auto.
-    - specialize (Abs n).
-      assert (absent_list (oss n)) as Abs'
-          by (apply Abs, EqNat.beq_nat_false; auto).
-      apply interp_vars_instant_sound in Vars as ->.
-      clear - Abs'; induction xs; simpl; auto.
-      inv Abs'; f_equal; auto.
-  Qed.
-
-  Lemma sub_inst_reset_memories:
-    forall F F' r x,
-      (forall k, sub_inst x (F k) (F' k)) ->
-      sub_inst x (reset_memories F r (F 0)) (reset_memories F' r (F' 0)).
-  Proof.
-    intros ** Sub.
-    pose proof (Sub 0) as Sub0.
-    eapply (sub_inst_reset_memories_path F r _ []) in Sub0.
-    unfold sub_inst, reset_memories.
-    rewrite Sub0; f_equal; simpl.
-    clear Sub0.
-    generalize (@nil ident).
-    induction (F' 0) as [?? IH] using memory_ind'; intros.
-    unfold reset_memories_path.
-    simpl. f_equal.
-    - f_equal.
-      extensionality y; extensionality mvs.
-      f_equal.
-      + extensionality n; unfold reset_content; simpl.
-        now rewrite Sub.
-      + extensionality n; unfold reset_reset; simpl.
-        now rewrite Sub.
-    - induction xms as [|(i & M')]; simpl; auto.
-      inversion_clear IH as [|?? Eq]; f_equal; auto.
-      f_equal.
-      unfold reset_memories_path in Eq; auto.
-  Qed.
-
-  (* Lemma foo: *)
-  (*   forall eqs M M', *)
-  (*     SemSB.well_structured_memories eqs M -> *)
-  (*     SemSB.well_structured_memories eqs M' -> *)
-  (*     (* SemSB.sem_equation P bk H M e -> *) *)
-  (*     (* SemSB.sem_equation P bk H M' e -> *) *)
-  (*     same_skeleton M M'. *)
-  (* Proof. *)
-  (*   intros ** WS WS'. *)
-  (*   revert dependent M'. *)
-  (*   induction M using memory_ind'; intros. *)
-  (*   constructor. *)
-  (*   - intros x Find. *)
-  (*     now apply WS, WS' in Find. *)
-  (*   - intros ** Find'. *)
-  (*     assert (find_inst x (Mnode xvs xms) <> None) as Find by (rewrite not_None_is_Some; eauto). *)
-  (*     apply WS, WS' in Find. *)
-  (*     apply not_None_is_Some in Find as (). *)
-  (*     eexists; split; eauto. *)
-  (*     unfold find_inst in Find'; *)
-  (*       apply Env.find_in, in_map with (f := snd) in Find'; simpl in Find'. *)
-  (*     eapply In_Forall in H; eauto. *)
-  (*     apply H. *)
-  (*     SearchAbout Forall In. *)
-  (*     eauto. *)
-  Definition gather_eq (acc: Env.t ident) (eq: SynSB.equation): Env.t ident :=
-    match eq with
-    | SynSB.EqDef _ _ _
-    | SynSB.EqReset _ _ _ _
-    | SynSB.EqFby _ _ _ _ => acc
-    | SynSB.EqCall _ _ f i _ => Env.add i f acc
-    end.
-
-  Definition gather (eqs: list SynSB.equation) : Env.t ident :=
-    fold_left gather_eq eqs [].
-
-  Arguments Env.add: simpl never.
-
-  Lemma fold_left_gather_eq_find:
-    forall eqs e e' x,
-      Env.find x e = Env.find x e' ->
-      Env.find x (fold_left gather_eq eqs e) = Env.find x (fold_left gather_eq eqs e').
-  Proof.
-    Arguments Env.add: simpl never.
-    unfold gather; induction eqs as [|eq]; simpl; auto; intros ** E.
-    destruct eq; simpl; auto.
-    apply IHeqs.
-    destruct (ident_eqb x i1) eqn: Eq;
-      [apply ident_eqb_eq in Eq; subst|apply ident_eqb_neq in Eq].
-    - rewrite 2 Env.gss; auto.
-    - rewrite 2 Env.gso; auto.
-  Qed.
-
-  Corollary gather_find:
-    forall eqs e x,
-      Env.find x e = None ->
-      Env.find x (fold_left gather_eq eqs e) = Env.find x (gather eqs).
-  Proof.
-    intros ** E; apply fold_left_gather_eq_find.
-    rewrite E; reflexivity.
-  Qed.
-
-  Lemma fold_left_gather_eq_find_not_none:
-     forall eqs e x,
-      Env.find x (fold_left gather_eq eqs e) <> None <->
-      Env.find x (gather eqs) <> None \/ Env.find x e <> None.
-  Proof.
-    unfold gather; induction eqs as [|eq]; simpl.
-    - split; intros E; auto.
-      destruct E; auto; discriminate.
-    - split; [intro E|intros [E|]]; rewrite IHeqs; try apply IHeqs in E as [|E]; auto.
-      + destruct eq; simpl gather_eq in *; auto.
-        destruct (ident_eqb x i1) eqn: Eq;
-          [apply ident_eqb_eq in Eq; subst|apply ident_eqb_neq in Eq].
-        * rewrite Env.gss in *; auto.
-        * rewrite Env.gso in E; auto.
-      + destruct eq; simpl gather_eq in *; try now contradict E.
-        destruct (ident_eqb x i1) eqn: Eq;
-          [apply ident_eqb_eq in Eq; subst|apply ident_eqb_neq in Eq].
-        * rewrite Env.gss in *; auto.
-        * rewrite Env.gso in E; auto; discriminate.
-      + destruct eq; simpl gather_eq in *; auto.
-        destruct (ident_eqb x i1) eqn: Eq;
-          [apply ident_eqb_eq in Eq; subst|apply ident_eqb_neq in Eq].
-        * rewrite Env.gss; right; discriminate.
-        * rewrite Env.gso; auto.
-  Qed.
-
-  Lemma fold_left_gather_eq_find_some:
-     forall eqs e x y,
-      Env.find x (fold_left gather_eq eqs e) = Some y <->
-      Env.find x (gather eqs) = Some y \/ (Env.find x e = Some y /\ Env.find x (gather eqs) = None).
-  Proof.
-    unfold gather; induction eqs as [|eq]; simpl.
-    - split; intros E; auto.
-      destruct E as [|()]; auto; discriminate.
-    - split; [intro E|intros ** [E|(?&E)]]; rewrite IHeqs; try apply IHeqs in E as [|(E & E')]; auto.
-      + destruct eq; simpl gather_eq in *; auto.
-        destruct (ident_eqb x i1) eqn: Eq;
-          [apply ident_eqb_eq in Eq; subst|apply ident_eqb_neq in Eq].
-        * rewrite Env.gss in *; auto.
-        * rewrite Env.gso in E; auto.
-          right; split; auto.
-          rewrite fold_left_gather_eq_find with (e' := []); auto.
-          apply Env.gso; auto.
-      + destruct eq; simpl gather_eq in *; try now contradict E.
-        destruct (ident_eqb x i1) eqn: Eq;
-          [apply ident_eqb_eq in Eq; subst|apply ident_eqb_neq in Eq].
-        * rewrite Env.gss in *; auto.
-        * rewrite Env.gso in E; auto; discriminate.
-      + destruct eq; simpl gather_eq in *; auto.
-        destruct (ident_eqb x i1) eqn: Eq;
-          [apply ident_eqb_eq in Eq; subst|apply ident_eqb_neq in Eq].
-        * contradict E.
-          rewrite fold_left_gather_eq_find_not_none.
-          right.
-          rewrite Env.gss; discriminate.
-        * rewrite Env.gso; auto.
-          right; split; auto.
-          erewrite fold_left_gather_eq_find; eauto.
-          rewrite Env.gso; auto.
-  Qed.
-
-  Lemma fold_left_gather_eq_find_none:
-     forall eqs e x,
-      Env.find x (fold_left gather_eq eqs e) = None <->
-      Env.find x (gather eqs) = None /\ Env.find x e = None.
-  Proof.
-    unfold gather; induction eqs as [|eq]; simpl.
-    - split; intros E; auto.
-      destruct E; auto.
-    - split; [intro E|intros ** (E&?)];
-        apply IHeqs in E as (E&E'); rewrite IHeqs;
-          destruct eq; simpl gather_eq in *; auto.
-      + split; [split|]; auto.
-        *{ destruct (ident_eqb x i1) eqn: Eq;
-            [apply ident_eqb_eq in Eq; subst|apply ident_eqb_neq in Eq].
-           - rewrite Env.gss in *; auto.
-           - rewrite Env.gso; auto.
-         }
-        *{ destruct (ident_eqb x i1) eqn: Eq;
-            [apply ident_eqb_eq in Eq; subst|apply ident_eqb_neq in Eq].
-           - rewrite Env.gss in *; discriminate.
-           - rewrite Env.gso in E'; auto.
-         }
-      + split; auto.
-        destruct (ident_eqb x i1) eqn: Eq;
-          [apply ident_eqb_eq in Eq; subst|apply ident_eqb_neq in Eq].
-        * rewrite Env.gss in *; discriminate.
-        * rewrite Env.gso in *; auto.
-  Qed.
-
-  Lemma gather_find':
-    forall eqs e x,
-      Env.find x (gather eqs) = None ->
-      Env.find x (fold_left gather_eq eqs e) = Env.find x e.
-  Proof.
-    intros ** E.
-    destruct (Env.find x e) eqn: E'.
-    - rewrite fold_left_gather_eq_find_some; auto.
-    - rewrite fold_left_gather_eq_find_none; auto.
-  Qed.
-
-  Lemma not_inst_in_gather_none:
-    forall eqs x,
-      ~ inst_in_eqs x eqs ->
-      Env.find x (gather eqs) = None.
-  Proof.
-    unfold gather; induction eqs as [|eq]; simpl; intros ** E; auto.
-    destruct eq; simpl gather_eq; try (now apply IHeqs; intro; apply E; right).
-      destruct (ident_eqb x i1) eqn: Eq;
-        [apply ident_eqb_eq in Eq; subst|apply ident_eqb_neq in Eq].
-    - exfalso; apply E.
-      left; constructor.
-    - rewrite fold_left_gather_eq_find_none; split.
-      + apply IHeqs; intro.
-        apply E; right; auto.
-      + rewrite Env.gso; auto.
-  Qed.
-
-  Lemma Welldef_gloabl_Is_well_sch:
-    forall G f n,
-      Welldef_global G ->
-      find_node f G = Some n ->
-      Is_well_sch (memories n.(n_eqs)) (map fst (n_in n)) n.(n_eqs).
-  Proof.
-    induction G as [|node]; intros ** WD Find.
-    - inv Find.
-    - inv WD.
-      simpl in Find.
-      destruct (ident_eqb node.(n_name) f); eauto.
-      inversion Find; subst n; auto .
-  Qed.
-
-  Lemma sub_inst_translate_sem_block:
-    forall G f bl P' M xss oss x M',
-      Welldef_global G ->
-      SemSB.sem_block (translate G) f M xss oss ->
-      SynSB.find_block f (translate G) = Some (bl, P') ->
-      sub_inst x M M' ->
-      exists g xss' oss',
-        SemSB.sem_block (translate G) g M' xss' oss'
-        /\ Env.find x (gather bl.(SynSB.b_eqs)) = Some g.
-  Proof.
-    intros ** WD Sem Find' Sub.
-    inversion_clear Sem as [????????? Find ????? Eqs WS].
-    rewrite Find in Find'; inv Find'.
-    apply find_block_translate in Find as (n & Find &?); subst; simpl in *.
-    assert (find_inst x M <> None) as E by (rewrite not_None_is_Some; eauto).
-    apply WS in E.
-    unfold SemSB.insts in E.
-    unfold translate_eqns, concatMap in *.
-    assert (compat_eqs n.(n_eqs)) as Compat.
-    { eapply Welldef_gloabl_Is_well_sch in WD; eauto.
-      eapply Is_well_sch_compat in WD; eauto.
-      eapply sem_equations_well_formed_app; eauto.
-    }
-    clear WD WS.
-    induction (n_eqs n) as [|eq].
-    - contradict E; apply not_In_empty.
-    - inversion_clear Compat as [|??? Compat_eq].
-      destruct eq; try destruct o as [()|]; unfold gather; simpl in *;
-        inversion_clear Eqs as [|?? Heq Heqs];
-        inv Compat_eq; auto.
-      + set (y := hd default i) in *.
-        inversion_clear Heqs as [|?? Heq''].
-        inversion_clear Heq'' as [| | |???????????? Sub'].
-        destruct (ident_eqb x y) eqn: Eq;
-          [apply ident_eqb_eq in Eq; subst|apply ident_eqb_neq in Eq].
-        *{ unfold sub_inst in Sub'; rewrite Sub in Sub'; inv Sub'.
-           do 3 eexists; split; eauto.
-           rewrite gather_find'.
-           - apply Env.gss.
-           - apply not_inst_in_gather_none; auto.
-         }
-        *{ rewrite gather_find.
-           - apply IHl; auto.
-             apply SemSB.In_fold_left_inst_eq in E as [|E]; auto.
-             rewrite 2 PSE.MP.Dec.F.add_neq_iff in E; auto.
-             contradict E; apply not_In_empty.
-           - rewrite Env.gso; auto.
-         }
-      + set (y := hd default i) in *.
-        inversion_clear Heq as [| | |???????????? Sub'].
-        destruct (ident_eqb x y) eqn: Eq;
-          [apply ident_eqb_eq in Eq; subst|apply ident_eqb_neq in Eq].
-        *{ unfold sub_inst in Sub'; rewrite Sub in Sub'; inv Sub'.
-           do 3 eexists; split; eauto.
-           rewrite gather_find'.
-           - apply Env.gss.
-           - apply not_inst_in_gather_none; auto.
-         }
-        *{ rewrite gather_find.
-           - apply IHl; auto.
-             apply SemSB.In_fold_left_inst_eq in E as [|E]; auto.
-             rewrite PSE.MP.Dec.F.add_neq_iff in E; auto.
-             contradict E; apply not_In_empty.
-           - rewrite Env.gso; auto.
-         }
-  Qed.
-
-  Lemma sem_block_same_skeleton:
-    forall G M M' f xss oss xss' oss',
-      (* Ordered_nodes G -> *)
-      Welldef_global G ->
-      SemSB.sem_block (translate G) f M xss oss ->
-      SemSB.sem_block (translate G) f M' xss' oss' ->
-      same_skeleton M M'.
-  Proof.
-    induction M as [?? IH] using memory_ind'.
-    intros ** Sem Sem'; pose proof Sem as Sem1; pose proof Sem' as Sem2;
-      inversion_clear Sem as [????????? Find ????? Eqs WS];
-      inversion_clear Sem' as [????????? Find' ????? Eqs' WS'].
-    rewrite Find' in Find; inv Find.
-    constructor.
-    - intros x E.
-      apply WS'.
-      apply WS in E; auto.
-    - intros ** E.
-      pose proof E as E1.
-      assert (find_inst x (Mnode xvs xms) <> None) as E' by (rewrite not_None_is_Some; eauto).
-      apply WS, WS' in E'.
-      apply not_None_is_Some in E' as ().
-      eexists; split; eauto.
-      unfold find_inst in E.
-      apply Env.find_in, in_map with (f := snd) in E; simpl in E.
-      eapply In_Forall in IH; eauto.
-      eapply sub_inst_translate_sem_block in Sem1 as (?&?&?&?& Find1); eauto.
-      eapply sub_inst_translate_sem_block in Sem2 as (?&?&?&?& Find2); eauto.
-      rewrite Find1 in Find2; inv Find2.
-      eauto.
-  Qed.
-
-  Lemma well_structured_reset_memories:
-    forall Fm r M0 eqs,
-    SemSB.well_structured_memories eqs M0 ->
-    SemSB.well_structured_memories eqs (reset_memories Fm r M0).
-  Proof.
-    inversion_clear 1 as [Vals Insts].
-    constructor; intro; unfold reset_memories, reset_memories_path.
-    - rewrite find_val_mmapi, <-Vals.
-      destruct (find_val x M0); simpl; split; auto; intros ** ?; discriminate.
-    - rewrite find_inst_mmapi, <-Insts.
-      destruct (find_inst x M0); simpl; split; auto; intros ** ?; discriminate.
-  Qed.
-
-  Ltac interp_sound n :=
-    repeat match goal with
-           | H: sem_var ?H' ?x ?vs |- _ =>
-             specialize (H n); apply sem_var_instant_reset in H
-           | H: sem_vars ?H' ?xs ?vss |- _ =>
-             specialize (H n); apply sem_vars_instant_reset in H
-           | H: sem_caexp ?bk ?H' ?c ?e ?vs |- _ =>
-             specialize (H n); simpl in H; eapply sem_caexp_instant_reset in H; eauto
-           | H: sem_laexp ?bk ?H' ?c ?e ?vs |- _ =>
-             specialize (H n); simpl in H; eapply sem_laexp_instant_reset in H; eauto
-           | H: sem_laexps ?bk ?H' ?c ?es ?vss |- _ =>
-             specialize (H n); simpl in H; eapply sem_laexps_instant_reset in H; eauto
-           end;
-    unfold interp_var, interp_vars, interp_laexp, interp_laexps, interp_caexp, lift, lift';
-    try erewrite <-interp_caexp_instant_sound;
-    try erewrite <-interp_laexp_instant_sound;
-    try erewrite <-interp_laexps_instant_sound;
-    try erewrite <-interp_var_instant_sound;
-    try erewrite <-interp_vars_instant_sound;
-    eauto.
-
-  (* Require Import Coq.Logic.ClassicalChoice. *)
-  (* Require Import Coq.Logic.ConstructiveEpsilon. *)
-  (* Require Import Coq.Logic.Epsilon. *)
-  Require Import Coq.Logic.IndefiniteDescription.
-
-  Theorem slices_sem_block:
-    forall G f r xss oss Fm,
-      Welldef_global G ->
-      (forall k,
-          SemSB.sem_block (translate G) f (Fm k)
-                          (mask (all_absent (xss 0)) k r xss)
-                          (mask (all_absent (oss 0)) k r oss)) ->
-      SemSB.sem_block (translate G) f (reset_memories Fm r (Fm 0)) xss oss.
-  Proof.
-    intros ** WD Sem.
-    revert dependent f; revert xss oss r Fm.
-    induction G as [|node]; intros.
-    specialize (Sem 0); inv Sem;
-      match goal with Hf: SynSB.find_block _ _ = _ |- _ => inversion Hf end.
-
-    pose proof (Welldef_global_Ordered_nodes _ WD) as Ord.
-    pose proof (Welldef_global_cons _ _ WD) as WD'.
-
-    pose proof Ord as Ord'.
-    inversion_clear Ord as [|?? Ord'' Hnneqs Hnn].
-
-    assert (exists bl P', SynSB.find_block f (translate (node :: G)) = Some (bl, P'))
-      as (bl & P' & Find)
-        by (specialize (Sem 0); inv Sem; eauto).
-
-    assert (forall k k', same_skeleton (Fm k) (Fm k')) as SameSkeleton
-        by (intros; pose proof (Sem k) as Sk; specialize (Sem k');
-            eapply sem_block_same_skeleton with (1 := WD); eauto).
-
-    assert (exists F, forall k, exists bk,
-                   sem_vars (F k) (map fst (SynSB.b_in bl)) (mask (all_absent (xss 0)) k r xss)
-                   /\ sem_vars (F k) (map fst (SynSB.b_out bl)) (mask (all_absent (oss 0)) k r oss)
-                   /\ Forall (SemSB.sem_equation (translate (node :: G)) bk (F k) (Fm k)) (SynSB.b_eqs bl)
-                   /\ clock_of (mask (all_absent (xss 0)) k r xss) bk
-                   /\ SemSB.well_structured_memories (SynSB.b_eqs bl) (Fm k))
-      as (Fh & Spec).
-    { assert (forall k, exists H bk,
-                   sem_vars H (map fst (SynSB.b_in bl)) (mask (all_absent (xss 0)) k r xss)
-                   /\ sem_vars H (map fst (SynSB.b_out bl)) (mask (all_absent (oss 0)) k r oss)
-                   /\ Forall (SemSB.sem_equation (translate (node :: G)) bk H (Fm k)) (SynSB.b_eqs bl)
-                   /\ clock_of (mask (all_absent (xss 0)) k r xss) bk
-                   /\ SemSB.well_structured_memories (SynSB.b_eqs bl) (Fm k))
-        as Spec.
-      { intro; specialize (Sem k); inv Sem.
-        match goal with
-          H: SynSB.find_block _ _ = _ |- _ => rewrite Find in H; inv H end.
-        eauto 7.
-      }
-      now apply functional_choice in Spec.
-    }
-
-    assert (forall x k n,
-               In x (map fst (SynSB.b_in bl) ++ map fst (SynSB.b_out bl)) ->
-               exists v, PM.find x (restr_hist (Fh k) n) = Some v)
-      as SameDomFh.
-    { clear - Spec.
-      intros ** Hin.
-      apply in_app in Hin as [Hin|Hin].
-      - destruct (Spec k) as (?& In & ?).
-        specialize (In n); simpl in *.
-        eapply Forall2_In_l in In as (?& Sem); eauto.
-        inv Sem; eauto.
-      - destruct (Spec k) as (?&?& Out &?).
-        specialize (Out n); simpl in *.
-        eapply Forall2_In_l in Out as (?& Sem); eauto.
-        inv Sem; eauto.
-    }
-
-    eapply SemSB.SBlock with (H := reset_history Fh r (Fh 0)); eauto.
-    - apply clock_of_equiv.
-    - intro; destruct (Spec (count r n)) as (?& In & ?).
-      eapply sem_var_instant_bl_vars; eauto.
-      intros ? ?; rewrite in_app; auto.
-    - intro; destruct (Spec (count r n)) as (?&?& Out &?).
-      eapply sem_var_instant_bl_vars; eauto.
-      intros ? ?; rewrite in_app; auto.
-    - intro; specialize (Sem (count r n)); inversion_clear Sem as [???????????? Same].
-      specialize (Same n); rewrite mask_transparent in Same; auto.
-    - intro; specialize (Sem (count r n)); inversion_clear Sem as [????????????? Same].
-      specialize (Same n); rewrite mask_transparent in Same; auto.
-    - intro; specialize (Sem (count r n)); inversion_clear Sem as [?????????????? AbsAbs].
-      specialize (AbsAbs n); rewrite 2 mask_transparent in AbsAbs; auto.
-    - assert (forall n, 0 < length (xss n)) as Length.
-      { clear - Sem.
-        pose proof Sem as Sem'.
-        intro; specialize (Sem 0); inversion_clear Sem as [?????????? Vars];
-          specialize (Vars n); simpl in Vars.
-        apply Forall2_length in Vars.
-        rewrite mask_length in Vars.
-        - rewrite <-Vars, map_length; apply SynSB.b_ingt0.
-        - eapply wf_streams_mask.
-          intro k'; specialize (Sem' k');
-            apply SemSB.sem_block_wf in Sem' as (); eauto.
-      }
-
-      assert (~ is_block_in (n_name node) (SynSB.b_eqs bl)) as NotIn.
-      { pose proof Find as Find'. simpl in Find.
-        destruct (ident_eqb (n_name node) f) eqn: E.
-        - assert (n_name node = SynSB.b_name bl) as -> by (inv Find; auto).
-          eapply find_block_not_is_block_in with (1 := Ord'); eauto.
-        - eapply find_block_later_not_is_block_in; eauto.
-      }
-
-      assert (forall k, exists bk,
-                   sem_vars (Fh k) (map fst (SynSB.b_in bl)) (mask (all_absent (xss 0)) k r xss)
-                   /\ sem_vars (Fh k) (map fst (SynSB.b_out bl)) (mask (all_absent (oss 0)) k r oss)
-                   /\ Forall (SemSB.sem_equation (translate (node :: G)) bk (Fh k) (Fm k)) (SynSB.b_eqs bl)
-                   /\ clock_of (mask (all_absent (xss 0)) k r xss) bk) as Spec'
-          by (intro; destruct (Spec k) as (?&?&?&?&?&?); eauto).
-      clear Spec; rename Spec' into Spec.
-
-      induction (SynSB.b_eqs bl) as [|eq ? IHeqs]; constructor; auto.
-      + clear IHeqs.
-        assert (forall k, exists bk, SemSB.sem_equation (translate (node :: G)) bk (Fh k) (Fm k) eq
-                           /\ clock_of (mask (all_absent (xss 0)) k r xss) bk)
-          as Spec'
-            by (intros; destruct (Spec k) as (?&?&?& Heq &?); inv Heq; eauto).
-        clear Spec.
-        set (bk := clock_of' xss).
-        set (H := reset_history Fh r (Fh 0)).
-
-        assert (spec_eq Fh eq) as SpecEq
-            by (eapply sem_spec_eq; intros; destruct (Spec' k) as (?&?&?); eauto).
-
-        destruct eq; inv SpecEq.
-
-        * apply SemSB.SEqDef with (xs := interp_caexp bk H c c0);
-            intro; destruct (Spec' (count r n)) as (?& Heq &?); inv Heq;
-              interp_sound n.
-
-        *{ apply SemSB.SEqFby with (xs := interp_var H i) (ls := interp_laexp bk H c l0);
-             try (intro; destruct (Spec' (count r n)) as (?& Heq &?); inv Heq; interp_sound n).
-           assert (exists F, forall k, exists bk xs ls,
-                          sem_var (Fh k) i xs
-                          /\ sem_laexp bk (Fh k) c l0 ls
-                          /\ find_val i (Fm k) = Some (F k)
-                          /\ (F k).(SemSB.content) 0 = sem_const c0
-                          /\ (forall n,
-                                match ls n with
-                                | absent =>
-                                  (F k).(SemSB.content) (S n) =
-                                  (if (F k).(SemSB.reset) (S n) then sem_const c0 else (F k).(SemSB.content) n)
-                                  /\ xs n = absent
-                                | present v' =>
-                                  (F k).(SemSB.content) (S n) =
-                                  (if (F k).(SemSB.reset) (S n) then sem_const c0 else v')
-                                  /\ xs n = present ((F k).(SemSB.content) n)
-                                end)
-                          /\ clock_of (mask (all_absent (xss 0)) k r xss) bk)
-             as (Fmvs & Spec).
-           { assert (forall k, exists mvs bk xs ls,
-                          sem_var (Fh k) i xs
-                          /\ sem_laexp bk (Fh k) c l0 ls
-                          /\ find_val i (Fm k) = Some mvs
-                          /\ mvs.(SemSB.content) 0 = sem_const c0
-                          /\ (forall n,
-                                match ls n with
-                                | absent =>
-                                  mvs.(SemSB.content) (S n) =
-                                  (if mvs.(SemSB.reset) (S n) then sem_const c0 else mvs.(SemSB.content) n)
-                                  /\ xs n = absent
-                                | present v' =>
-                                  mvs.(SemSB.content) (S n) =
-                                  (if mvs.(SemSB.reset) (S n) then sem_const c0 else v')
-                                  /\ xs n = present (mvs.(SemSB.content) n)
-                                end)
-                          /\ clock_of (mask (all_absent (xss 0)) k r xss) bk) as Spec.
-             { intro; destruct (Spec' k) as (?& Heq &?); inversion_clear Heq as [|??????????? Fby| |]; inv Fby.
-               eauto 10.
-             }
-             now apply functional_choice in Spec.
-           }
-
-           apply SemSB.mfby_intro with (mvs := reset_mvalues Fmvs r).
-           - apply find_val_reset_memories.
-             intro; destruct (Spec k) as (?&?&?&?); intuition.
-           - simpl; destruct (r 0).
-             + destruct (Spec 1) as (?&?&?&?); intuition.
-             + destruct (Spec 0) as (?&?&?&?); intuition.
-           - intro; destruct (Spec (count r n)) as (?&?&?&?&?&?&?& Heq &?).
-             pose proof (reset_mvalues_spec _ _ _ _ _ _ _ _ _ Length Spec (S n)) as SpecMv.
-             clear Spec.
-             interp_sound n.
-             specialize (Heq n).
-             destruct (r (S n)) eqn: E;
-               [rewrite SpecMv; auto|];
-               simpl; rewrite E; simpl; auto.
-             destruct (x1 n); intuition.
-         }
-
-        *{ assert (exists M0, sub_inst i0 (Fm 0) M0) as (M0 & Find0)
-               by (destruct (Spec' 0) as (?& Heq & ?); inv Heq; eauto).
-           apply SemSB.SEqReset with (rs := interp_var H i1) (M' := reset_memories_path Fm r [i0] M0).
-           - intro; destruct (Spec' (count r n)) as (?& Heq &?); inv Heq; interp_sound n.
-           - now apply sub_inst_reset_memories_path.
-           - rewrite reset_regs_instant_spec.
-             intro; destruct (Spec' (count r n)) as (?& Heq &?); inversion_clear Heq as [| |????????? Var|].
-             eapply reset_memories_path_sub_spec_instant'; eauto.
-             + eapply same_skeleton_sub_inst; eauto.
-             + replace (reset_of (interp_var H i1) n) with (reset_of_value (interp_var H i1 n)); auto.
-               interp_sound n.
-               replace (reset_of_value (rs n)) with (reset_of rs n); auto.
-               apply reset_regs_instant_spec'; auto.
-         }
-
-        *{ assert (exists F, (forall k,
-                            SemSB.sem_block (translate G) i0
-                                            (F k)
-                                            (mask (all_absent (interp_laexps bk H c l0 0)) k r (interp_laexps bk H c l0))
-                                            (mask (all_absent (interp_vars H i 0)) k r (interp_vars H i)))
-                        /\ forall k, sub_inst i1 (Fm k) (F k)) as (F & Spec & Sub).
-           { assert (forall k, exists M bk ess oss,
-                          sem_laexps bk (Fh k) c l0 ess
-                          /\ sub_inst i1 (Fm k) M
-                          /\ SemSB.sem_block (translate (node :: G)) i0 M ess oss
-                          /\ sem_vars (Fh k) i oss
-                          /\ clock_of (mask (all_absent (xss 0)) k r xss) bk) as Spec.
-             { intro; destruct (Spec' k) as (?& Heq & Clock);
-                 inversion_clear Heq as [| | |???? M' ?????? Exps ? Block Vars]; eauto 9.
-             }
-             apply functional_choice in Spec as (F & Spec).
-             exists F; split; intro; destruct (Spec k) as (?&?&?& Exps & ? & Block & Vars & ?); auto.
-             erewrite sem_laexps_interp_mask in Block; eauto.
-             pose proof Block as Block'; inversion_clear Block' as [?????????????? Same].
-             destruct (Spec' 0) as (?& Heq &?); inv Heq.
-             erewrite sem_vars_interp_mask with (1 := Vars) (r := r) in Block; eauto.
-             - eapply sem_block_cons; eauto.
-               intro E; apply NotIn; rewrite E; do 2 constructor.
-             - intros ** E; apply Same.
-               rewrite mask_opaque; auto.
-               apply all_absent_spec.
-           }
-           eapply SemSB.SEqCall with (M' := reset_memories F r (F 0))
-                                     (ess := interp_laexps bk H c l0)
-                                     (oss := interp_vars H i).
-           - intro; destruct (Spec' (count r n)) as (?& Heq &?); inv Heq; interp_sound n.
-           - now apply sub_inst_reset_memories.
-           - apply sem_block_cons2; auto.
-           - intro; destruct (Spec' (count r n)) as (?& Heq &?); inv Heq; interp_sound n.
-         }
-
-      + apply IHeqs.
-        * intro E; apply NotIn; right; auto.
-        * intro; destruct (Spec k) as (?&?&?& Heqs &?); inv Heqs; eauto.
-
-    - destruct (Spec 0) as (?&?&?&?&?&?).
-      apply well_structured_reset_memories; auto.
-  Qed.
-
-  Theorem reset_correctness:
-    forall G f r xss oss,
-      Welldef_global G ->
-      (forall f xss oss,
-          sem_node G f xss oss ->
-          exists M, SemSB.sem_block (translate G) f M xss oss) ->
-      sem_reset G f r xss oss ->
-      exists M, SemSB.sem_block (translate G) f M xss oss
-           /\ SemSB.reset_regs r M.
-  Proof.
-    intros ** Ord IHNode Sem.
-    inversion_clear Sem as [???? Sem'].
-
-    assert (exists F, forall k, SemSB.sem_block (translate G) f (F k)
-                                      (mask (all_absent (xss 0)) k r xss)
-                                      (mask (all_absent (oss 0)) k r oss))
-      as (Fm & Sem).
-    { assert (forall k, exists M', SemSB.sem_block (translate G) f M'
-                                         (mask (all_absent (xss 0)) k r xss)
-                                         (mask (all_absent (oss 0)) k r oss)) as SBsem
-          by (intro; specialize (Sem' k); apply IHNode in Sem'; auto).
-
-      (** Infinite Description  *)
-      now apply functional_choice in SBsem.
-
-      (** Epsilon  *)
-      (* assert (inhabited memories) as I *)
-      (*     by (constructor; exact (fun n => @empty_memory val)). *)
-      (* exists (fun n => epsilon *)
-      (*            I (fun M => msem_node G f (mask (all_absent (xs 0)) n r xs) M *)
-      (*                               (mask (all_absent (ys 0)) n r ys))). *)
-      (* intro; now apply epsilon_spec.  *)
-
-      (** Constructive Epsilon  *)
-      (* pose proof (constructive_ground_epsilon memories) as F. *)
-
-      (** Classical Choice  *)
-      (* now apply choice in Msem'.   *)
-    }
-    apply slices_sem_block in Sem; eauto.
-  Qed.
-
-  Theorem correctness:
-    forall G f xss oss,
-      Welldef_global G ->
-      sem_node G f xss oss ->
-      exists M, SemSB.sem_block (translate G) f M xss oss.
-  Proof.
-    induction G as [|node].
-    inversion 2;
-      match goal with Hf: find_node _ [] = _ |- _ => inversion Hf end.
-    intros ** WD Hsem.
-    assert (Hsem' := Hsem).
-    inversion_clear Hsem' as [??????? Hfind ????? Heqs].
-    pose proof (Welldef_global_Ordered_nodes _ WD) as Hord.
-    pose proof (Welldef_global_cons _ _ WD) as WD'.
-    pose proof (find_node_not_Is_node_in _ _ _ Hord Hfind) as Hnini.
-    simpl in Hfind.
-    destruct (ident_eqb node.(n_name) f) eqn:Hnf.
-    - assert (Hord':=Hord).
-      inversion_clear Hord as [|? ? Hord'' Hnneqs Hnn].
-      inv Hfind.
-      eapply Forall_sem_equation_global_tl in Heqs; eauto.
-
-      assert (forall f xss oss,
-                 sem_node G f xss oss ->
-                 exists M, SemSB.sem_block (translate G) f M xss oss)
-        as IHG' by auto.
-
-      assert (forall f r xss oss,
-                 sem_reset G f r xss oss ->
-                 exists M, SemSB.sem_block (translate G) f M xss oss
-                      /\ SemSB.reset_regs r M)
-        by (intros; apply reset_correctness; auto).
-
-      assert (exists M', Forall (SemSB.sem_equation (translate G) bk H M') (translate_eqns n.(n_eqs))
-                    /\ SemSB.well_structured_memories (translate_eqns n.(n_eqs)) M')
-        as (M & Hmsem & WS).
-      { eapply equations_correctness; eauto.
-        inv WD; eapply Is_well_sch_compat; eauto.
-        eapply nl_sem_equations_well_formed_app; eauto.
-      }
-
-      exists M.
-      econstructor; eauto.
-      + simpl; now rewrite Hnf.
-      + simpl; rewrite map_fst_idty; eauto.
-      + simpl; rewrite map_fst_idty; eauto.
-      + eapply sem_equation_cons; eauto.
-      + auto.
-    - apply ident_eqb_neq in Hnf.
-      eapply sem_node_cons in Hsem; eauto.
-      inv Hord.
-      eapply IHG in Hsem as [M]; eauto.
-      exists M.
-      now eapply sem_block_cons2; eauto.
-  Qed.
